【详解】解：如图，过点 $A . B$ 作 $A F \perp y$ 轴于点 $F$ ， $A D \perp x$ 轴于点 $D$ ， $B E \bot x$ 于点 $E$ ，

![](<../../qs_image_DB/专题1-4_一文搞定反比例函数7个模型，13类题型（解析版）_/530f519bb84b6eea19904bf33fa672bc871ebaac2949e19390c6e83bae7f38b4.jpg>)

$: S _ { { \overline { { \substack { \scriptstyle { \mathrm { \tiny ~ \frac { 1 } } { \scriptstyle { \mathrm { \tiny ~ \frac { 1 } } { \scriptstyle { \mathrm { \tiny ~ \frac { 1 } } { \scriptstyle { \mathrm { \tiny ~ \frac { 1 } } } { \scriptstyle { \mathrm { \tiny ~ \frac { 1 } } { \scriptstyle { \mathrm \ddots } } } } } } } } } } } } } } } = S _ { { \mathrm { \tiny ~ \frac { _ { \scriptstyle \mathrm { \tiny ~ \ A F O } } } } } } + S _ { { \mathrm { \tiny ~ \frac { _ { \scriptstyle \mathrm { \tiny ~ \ A B O } } } } } } + S _ { { \mathrm { \tiny ~ \frac { _ { \scriptstyle \Delta B O E } } } } } = k + 6$ $S _ { \textmd { ‰} } = S _ { \textmd { \textmu \textmu \textmu \textmu \textit {  } } } + S _ { \textmu \textmu \textit { \textmu \textmu \textit {  } } } = k + S _ { \textmu \textmu \textit { \textmu \textmu \textit {  } } }$ ADEB  S 梯形 6    
$\begin{array} { l } { \displaystyle \therefore \frac { ( y _ { 2 } + y _ { 1 } ) ( x _ { 2 } - x _ { 1 } ) } { 2 } = 6 } \\ { \displaystyle \because x _ { 2 } = 2 x _ { 1 } } \end{array}$

【淘宝店铺：向阳百分百】 2 112 y  y
$\therefore { \frac { ( y _ { 2 } + y _ { 1 } ) ( x _ { 2 } - x _ { 1 } ) } { 2 } } = { \frac { ( { \frac { 1 } { 2 } } y _ { 1 } + y _ { 1 } ) ( 2 x _ { 1 } - x _ { 1 } ) } { 2 } } = { \frac { 3 } { 4 } } y _ { 1 } x _ { 1 } = 6$   
 x1y1=8   
 k  8   
$S _ { \scriptscriptstyle \mathrm { s } A B C } = \frac { 1 } { 2 } A C { \ P } C \quad \frac { 1 } { 2 } ( x _ { 2 } - \ x _ { 1 } ) \ P ( y _ { 1 } \quad y _ { 2 } ) = \frac { 1 } { 2 } x _ { 1 } \ P \frac { 1 } { 2 } y _ { 1 } \quad \frac { 1 } { 4 } x _ { 1 } y _ { 1 } = \frac { 1 } { 4 } { \ P } \quad 2 \quad \frac { 1 } { 8 } \quad \frac { 1 } { 2 } x _ { 2 } = \frac { 1 } { 8 } \quad 2 \quad \frac { 1 } { 8 } \quad \frac { 1 } { 2 } x _ { 1 } = 0 .$
