【详解】解：∵ $y = n x + 4 n - 6$ ，$y = n { \bigl ( } x + 4 { \bigr ) } - 6$ ，  
当 $x = - 4$ 时， $y = - 6$ ，即一次函数 $y = n x + 4 n - 6$ 经过点 $\left( - 4 , - 6 \right)$ ，  
∵y 关于 $x$ 的一次函数 $y = n x + 4 n - 6$ 图象上存在 $_ n$ 阶积点”，  
设点 $\left( x , y \right)$ 是一次函数 $y = n x + 4 n - 6$ 图象上的 $\cdot$ 阶积点”，  
∴ $\left| x \right| \cdot \left| y \right| = n$ ，则 $n > 0$ ，  
∴ $\left| y \right| = \frac { n } { \left| x \right| }$ 一次函数 $y = n x + 4 n - 6$ 经过一、三象限，$y = { \frac { n } { x } }$ 或 y  $y = - { \frac { n } { x } }$ $y = { \frac { n } { x } }$ 经过一、三象限，一次函数 $y = n x + 4 n - 6$ 经过一、三象限，$y = { \frac { n } { x } }$ 函数图象与 $y = n x + 4 n - 6$ 函数图象有 2 个交点；$\cdot _ { y }$ 关于 $x$ 的一次函数 $y = n x + 4 n - 6$ 图象的 $^ { * } n$ 阶积点”恰好有 3 个，$y = - { \frac { n } { x } }$ 函数图象与 $y = n x + 4 n - 6$ 函数图象有 1 个交点，  
联立得： $\left\{ \begin{array} { l l } { \displaystyle y = - \frac { n } { x } } \\ { \displaystyle y = n x + 4 n - 6 } \end{array} \right.$ ,  
则 $- { \frac { n } { x } } = n x + 4 n - 6$ ，  
整理得： $n x ^ { 2 } + ( 4 n - 6 ) x + n = 0$ ，  
$\therefore \Delta = b ^ { 2 } - 4 a c = \left( 4 n - 6 \right) ^ { 2 } - 4 n ^ { 2 } = 0$ ，解得： $n = 1$ 或 3
