【详解】（1）将 $A \left( - 3 , 0 \right)$ ， $B \mathopen { } \mathclose \bgroup \left( 6 , 0 \aftergroup \egroup \right)$ 代入 $y = a x ^ { 2 } + b x - 9$ ，得 $\left\{ \begin{array} { l l } { 9 a - 3 b - 9 = 0 } \\ { 3 6 a + 6 b - 9 = 0 } \end{array} \right.$ 解得 $\left\{ { \begin{array} { l } { \displaystyle a = { \frac { 1 } { 2 } } } \\ { \displaystyle b = - { \frac { 3 } { 2 } } } \end{array} } \right.$

∴抛物线解析式为： $y = { \frac { 1 } { 2 } } x ^ { 2 } - { \frac { 3 } { 2 } } x - 9$ （2）如图，过点 $D$ 作 $D G \bot A B$ ，过点 $E$ 作 $E F \perp A B$ ，垂足为 $\cdot$ ， $\cdot$ ，

![](<../../qs_image_DB/专题2-7_二次函数中的最值问题（解析版）/037d8f46c8fb38e26eba9b489b16c4b40b0dd5c31f64814c0599342b439a57db.jpg>)

$P E / / B C$ ， $P D \perp B C$ $\therefore \mathrm { D } D P E = \mathrm { \ D } P D B = \mathrm { \ } 9 0 ^ { \circ }$ $\textcircled { 1 } F P E + \textcircled { 1 } D P B = 9 0 ^ { \circ }$ $\cdot \cdot \mathrm { \nabla } \mathrm { \sf ~ D } D P B + \mathrm { \nabla } \mathrm { \sf ~ D } B P = 9 0 ^ { \circ }$ $\dot { \cdot } \mathrm { ~ D ~ } F P E = \mathrm { ~ D ~ } D B P$ ，同理可得 $\Game P D G = \ G D B P$ 设直线 $A C$ 的解析式为： $y = k x + h$ 则 $\displaystyle { \left\{ - 3 k + h = 0 \right. }$ 解得 $\left\{ \begin{array} { l } { k = - 3 } \\ { h = - 9 } \end{array} \right.$ ∴直线 $\begin{array} { r l } { A C } & { { } { }  y = - 3 x - 9 } \end{array}$ 同理由点 $B ( 6 , 0 )$ ， $C ( 0 , - 9 )$ ，可求得直线 $B C$ ： $y = \frac { 3 } { 2 } x - 9$ 设点 $E ( p , - 3 p - 9 )$ ， $D ( q , \frac { 3 } { 2 } q - 9 )$ ，则 $\quad = \ m - \ p \quad P G = \ q ^ { - } \ m E F = \ 3 p ^ { + } \ 9 \quad D G = - \ \frac { 3 } { 2 } q ^ { + } \ 9$ $\mathrm { R t } _ { \Delta B O C }$ 中， $O B = 6 O C = 9$ $B C = { \sqrt { O C ^ { 2 } + O B ^ { 2 } } } = { \sqrt { 6 ^ { 2 } + 9 ^ { 2 } } } = { \sqrt { 1 1 7 } }$ ∴ tan Ð OBC = $O B C = \frac { 9 } { 6 } = \frac { 3 } { 2 }$ ,$\mathrm { R t } \triangle P E F$ 中， tan $\mathrm { ~ ) ~ } F P E = \frac { E F } { P F } { = \tan \mathrm { ~ } \mathrm { ~ } O B C = \frac { 3 } { 2 } }$ $\frac { 3 p + 9 } { m - p } = \frac { 3 } { 2 }$ 2 解得 $p = \frac { 1 } { 3 } ( m - 6 )$ ，$P F = \ m - \ p = \ { \frac { 2 } { 3 } } ( m + \ 3 )$ $\therefore \cos \oplus F P E = { \frac { P F } { P E } } = \cosh O B C = { \frac { O B } { B C } } = { \frac { 6 } { \sqrt { 1 1 7 } } }$

$P E = \ P F \bullet { \frac { \sqrt { 1 1 7 } } { 6 } } = \frac { \sqrt { 1 1 7 } } { 9 } ( m + \ 3 )$   
$\mathbb { R } { \mathrm { t } } \triangle P D G$ 中， tan Ð $P D G = { \frac { P G } { D G } } { = }$ tan Ð $O B C = \frac { 3 } { 2 }$   
$\therefore \frac { q - m } { - \frac { 3 } { 2 } q + 9 } = \frac { 3 } { 2 }$ ，解得， $q = \frac { 1 } { 1 3 } ( 4 m + 5 4 )$   
$P G = q - m = - \frac { 9 } { 1 3 } ( m - 6 )$   
$\sin \beta P D G = { \frac { P G } { P D } } = \sin \beta O B C = { \frac { 9 } { \sqrt { 1 1 7 } } }$   
$\therefore P D = P G \bullet { \frac { \sqrt { 1 1 7 } } { 9 } } = - \ { \frac { \sqrt { 1 1 7 } } { 1 3 } } ( m ^ { - } \ 6 )$   
$\therefore S _ { \scriptscriptstyle  { s } P D D E } = \frac { 1 } { 2 } P D \bullet P E = \frac { 1 } { 2 } \bullet \frac { \sharp \widehat { \vec { \textbf { k } } } } { \lVert \boldsymbol { \nabla } \rVert } \frac { 1 1 7 } { 1 3 } ( m - \textbf { 6 } ) \bullet \frac { \sqrt { 1 7 } } { 9 } ( m + \textbf { 3 } ) = - \ \frac { 1 } { 2 } ( m + \textbf { 3 } ) ( m - \textbf { 6 } )$ ，  
即 PDES $S _ { _ { \Delta P D E } } = - \frac { 1 } { 2 } ( m ^ { + } \ 3 ) ( m ^ { - } \ 6 ) = - \frac { 1 } { 2 } ( m ^ { - } \ \frac { 3 } { 2 } ) ^ { 2 } + 1 0 \frac { 1 } { 8 }$   
$\cdot - \frac { 1 } { 2 } < 0$ $m = \frac { 3 } { 2 }$ 时， $- 3 < m < 6$ ， $S _ { \triangle P D E }$ 有最 大值 ，最 大值 为 $1 0 \frac { 1 } { 8 }$

# 2022·湖北襄阳中考真题
