【答案】 $\left( 2 { \sqrt { 2 } } - 2 , 0 \right) \ \left( - 2 + 2 { \sqrt { 2 } } , 0 \right)$

【分析】如图：过点 $\cdot$ 作 $C B ^ { \prime } \bot B C$ 使 $C B ^ { \prime } = A B$ ，连接 $B ^ { \prime } D$ ；证 $\triangle A B E \cong \triangle C B ^ { \prime } D ( \mathrm { S A S } )$ 可得 $D B ^ { \prime } = B E$ ，$A B = C B ^ { \prime }$ ；将 $A D + B E$ 最小值可转化成 $A D + C B ^ { \prime }$ 最小值，则当 $\cdot$ 、 $\cdot$ 、 $B$ 在同一直线上时， $A D + B E$ 最小，即 $A B ^ { \prime }$ 长度；；再根据 $A C = 2 \sqrt { 2 }$ 求得 $A B = C B ^ { \prime } = A C = 2 \sqrt { 2 }$ 、 $O A = O C = { \frac { \sqrt { 2 } } { 2 } } \times 2 { \sqrt { 2 } } = 2$ ，即$A { \big ( } 0 , 2 { \big ) } , B ^ { \prime } { \Big ( } 2 , - 2 { \sqrt { 2 } } { \Big ) }$ ；再运用待定系数法求得直线 $A B ^ { \prime }$ 表达式，最后将 $y = 0$ 代入表达式求得 $\cdot$ 的值即可解答
