【详解】方法一：过 $C$ 作 $C F \bot A C$ 于 $F$ ，使 $C F = 2 A C = 4$ ，连接 $E F$ 、 $B F$ ，
![](<../../qs_image_DB/专题2-6__逆等线之乾坤大挪移（解析版）/576f2c66c2428866662f63be67960ad44c4037504688d704d60ae0fc7896affe.jpg>)
∵ $C E = 2 A D$ ，  
$\therefore { \frac { C E } { A D } } = { \frac { C F } { A C } } = 2 \ ,$   
∵ $\angle D A C = \angle F A C = 9 0 ^ { \circ }$ ，  
$\therefore \Delta D A C \sim \Delta E C F$ ，$\frac { C E } { A D } = \frac { C F } { A C } = \frac { E F } { C D } = 2$ ，即 $E F = 2 C D$ ，  
$B E + 2 C D = B E + E F \geq B F$   
∴当 $B .$ 、E、 $F$ 三点共线时 $B E + 2 C D$ 有最小值，最小值为 $B F$ 的长  
∵ $\cdot \angle D A C = \angle F A C = 9 0 ^ { \circ }$   
$\therefore A B / / C F$ ，  
${ \frac { O B } { O F } } { = } { \frac { O A } { O C } } { = } { \frac { A B } { C F } }$   
$A B = 1 A C = 2 C F = 2 A C = 4$   
$\therefore { \frac { O B } { O F } } = { \frac { O A } { O C } } = { \frac { A B } { C F } } = { \frac { 1 } { 4 } } ,$   
$B F = \frac { 5 } { 4 } O F , O C = \frac { 4 } { 5 } A C = \frac { 8 } { 5 }$   
$O F = { \sqrt { O C ^ { 2 } + C F ^ { 2 } } } = { \sqrt { \left( { \frac { 8 } { 5 } } \right) ^ { 2 } + 4 ^ { 2 } } } = { \frac { 4 } { 5 } } { \sqrt { 2 9 } }$ ，  
$\therefore B F = { \frac { 5 } { 4 } } O F = { \sqrt { 2 9 } }$   
$B E + 2 C D$ 的最小值为 $\sqrt { 2 9 }$
方法二： $A D = x$ ，则 $C E = 2 A D = 2 x$ ， $A E = A C - C E = 2 - 2 x$ ，
![](<../../qs_image_DB/专题2-6__逆等线之乾坤大挪移（解析版）/abc370c0d46931a476d409976a91f3fe06f32cae75190f2aa473647bf6095b10.jpg>)
$B E = { \sqrt { A E ^ { 2 } + A B ^ { 2 } } } = { \sqrt { \left( 2 - 2 x \right) ^ { 2 } + 1 ^ { 2 } } } C D = { \sqrt { A D ^ { 2 } + A C ^ { 2 } } } = { \sqrt { x ^ { 2 } + 2 ^ { 2 } } }$   
设 $2 y = B E + 2 C D$ ，  
${ \begin{array} { l } { \displaystyle \therefore y = { \frac { 1 } { 2 } } B E + C D = { \frac { 1 } { 2 } } { \sqrt { \left( 2 - 2 x \right) ^ { 2 } + 1 ^ { 2 } + { \sqrt { x ^ { 2 } + 2 ^ { 2 } } } } } = { \sqrt { \left( x - 1 \right) ^ { 2 } + { \frac { 1 } { 4 } } + { \sqrt { x ^ { 2 } + 4 } } } } } \\ { = { \sqrt { \left( x - 1 \right) ^ { 2 } + \left( 0 - { \frac { 1 } { 2 } } \right) ^ { 2 } + { \sqrt { \left( x - 0 \right) ^ { 2 } + \left( 0 + 2 \right) ^ { 2 } } } } } } \end{array} }$   
∴y可以看成点 $M \left( x , 0 \right)$ 到点 $A { \bigg ( } 1 , { \frac { 1 } { 2 } } { \bigg ) } B { \big ( } 0 , - 2 { \big ) }$ 的距离之和，  
∴当 $M \left( x , 0 \right)$ 、 $A { \left( 1 , \frac { 1 } { 2 } \right) }$ 、 $B ( 0 , - 2 )$ 三点共线时 $y$ 最小 ，最 小值 $y = A B = { \sqrt { \left( 0 - 1 \right) ^ { 2 } + \left( - 2 - { \frac { 1 } { 2 } } \right) ^ { 2 } } } = { \frac { \sqrt { 2 9 } } { 2 } }$
