【详解】解：由图可知，当 $\cdot$ 时， $_ \mathrm { A E + C D = A B + A C = 2 }$   
∴A $scriptstyle { \mathrm { . B } } = { \mathrm { A C } } = 1$ ， $\mathrm { B C } { = } \sqrt { 2 }$ ，图象最低点函数值即为 $\mathrm { A E ^ { + C D } }$ 的最小值  
由题意可得： $\sqrt { x ^ { 2 } + 1 } \qquad \sqrt { \left( \frac { \sqrt { 2 } } { 2 } - x \right) ^ { 2 } + \left( \frac { \sqrt { 2 } } { 2 } \right) ^ { 2 } }$   
$\therefore \mathrm { A E + C D } = \sqrt { x ^ { 2 } + 1 } + \sqrt { ( \frac { \sqrt { 2 } } { 2 } - x ) ^ { 2 } + ( \frac { \sqrt { 2 } } { 2 } ) ^ { 2 } }$ 即点（x，0）到（0,-1）与 $( { \frac { \sqrt { 2 } } { 2 } } , { \frac { \sqrt { 2 } } { 2 } } )$ 的距离之和  
∴当这三点共线时， $\cdot$ 最小  
设该直线的解析式为 $\scriptstyle { \mathrm { y = k x + b } }$   
$\left\{ { \frac { - 1 = b } { 2 } } = { \frac { \sqrt { 2 } } { 2 } } k + b \right. \qquad $ 解得 $\scriptstyle { \left\{ \begin{array} { l l } { k = { \sqrt { 2 } } + 1 } \\ { b = - 1 } \end{array} \right. }$   
$\therefore y = \left( { \sqrt { 2 } } + 1 \right) x - 1$   
当 $\cdot$ 时， $\mathbf { x } { = } \sqrt { 2 } - 1$
