【详解】解：如图所示，延长 $B D$ 至 $F$ 使 $D F = B D$ ，作 $A G / / B C$ 交 $D F$ 于 $G$ ，

![](<../../qs_image_DB/专题1-1_一网打尽全等三角形模型_·十个模型（解析版）/7eab4a8ea62f177cfb98d3b223f4a36b244afb96de2d6f1f4b5135cbe221906e.jpg>)

 $B D = D F$ ， $A D \perp B E$ ，  
AF  AB， $\angle F = \angle A B D$ ，$\cdot A G / / B C$ ，  
 $\angle A G D = \angle E B C$ ， $\angle G A E = \angle C$ ，  
 $E B = E C$ ， ,  
 $\angle E B C = \angle C$ ，$. \angle C = \angle E B C = \angle A G D = \angle G A E$ ，  
 AE  EG ，  
 $\angle C = 2 \angle A B E$ ，$\angle A G D = 2 \angle A B E = 2 \angle F$ ，  
FG  AG ，  
 AC  22 ， BD 16，  
$\therefore B G = B E + G E = C E + A E = A C = 2 2 { \mathrm { ~ , } }$ ，  
$\therefore A G = F G = B F - B D = 2 B D - B G = 2 \times 1 6 - 2 2 = 1 0 ,$ ，$\therefore D G = D F - F G = 1 6 - 1 0 = 6$ ，  
$\therefore A D = { \sqrt { A G ^ { 2 } - D G ^ { 2 } } } = { \sqrt { 1 0 ^ { 2 } - 6 ^ { 2 } } } = 8$ ，

$$
\therefore A B = \sqrt { A D ^ { 2 } + B D ^ { 2 } } = \sqrt { 8 ^ { 2 } + 1 6 ^ { 2 } } = 8 \sqrt { 5 }
$$

# 提高篇
