【解析】证明：（1）∵AD∥BC，∴ $-$ ， $\angle C A D = \angle A C B$   
∵ $A B { = } A C$ ， $\cdot$ ， $\angle A B C = \angle A C B$ ，$-$   
∵ $\cdot _ { A D } = _ { A D }$ ，∴△ADE≌△ADC  
（2） $\cdot$   
在 $H B$ 上截取 $H F { = } H E$ ，连接 $D F$   
则 $\cdot$ ， $\therefore \angle E = \angle D F A$   
∵△ADE≌△ADC， $\therefore \angle E { = } \angle A C D$ ， $\cdot$ ，  
∴ $\angle D F A = \angle A C D$ ．  
∵ $-$ ，∴ $\angle D F A = 2 \angle A B D$ ，$-$ ， $\therefore B F = D F = D E = C D$ ，$-$ ，  
∴BF＝2AH， $\_$   
（3）∵ $\cdot C D = 6 , \therefore A H = 3 , E D = 6 ,$ ，$\begin{array} { c c } { { } } & { { } } \\ { { } } & { { 2 \sqrt { 5 } \qquad } } \end{array}$ ，$-$ ，$-$
