例20 请解答以下各题：
$\therefore B M = \sqrt { A B ^ { 2 } - A M ^ { 2 } } = \sqrt { 5 ^ { 2 } - 3 ^ { 2 } } = 4 ,$ ，  
在 $\mathrm { R t } _ { \triangle A C M }$ 中， $A C = { \sqrt { 1 0 } }$ ， $A M = 3$ ，  
$\therefore C M = \sqrt { A C ^ { 2 } - A M ^ { 2 } } = \sqrt { 1 0 - 3 ^ { 2 } } = 1 ,$ ，  
过点 $\cdot$ 作 $E P \perp A N$ 交 $A N$ 的延长线于 $\cdot$ ，过点 $\cdot$ 作 $G Q \bot A M$ 于 $\mathcal { Q }$ ，∵四边形ABDE是正方形，  
$\angle B = A E , \angle B A E = 9 0 ^ { \circ }$ ，  
$\angle E A P + \angle B A M = 1 8 0 ^ { \circ } - 9 0 ^ { \circ } = 9 0 ^ { \circ }$ ，$\therefore A M \bot B C$ ，  
$\angle A B M + \angle B A M = 9 0 ^ { \circ }$ ，  
$\dot { \cdot } \angle A B M = \angle E A P$ ，  
在 $\triangle A B M$ 和 $\triangle E A P$ 中，  
$\left\{ \begin{array} { l l } { \angle A B M = \angle E A P } \\ { \angle A M B = \angle P } \\ { A B = A E } \end{array} \right.$   
$\triangle A B M { \cong } \triangle E A P \big ( \mathrm { A A S } \big )$   
$\therefore E P = A M , A P = B M = 4 ,$   
同理可得 $G Q = A M$ ，  
$E P = G Q$ ；  
在△EPN 和 $\triangle G Q N$ 中，  
$\left\{ \begin{array} { l l } { \angle P = \angle N Q G } \\ { \angle E N P = \angle G N Q } \\ { E P = G Q } \end{array} \right.$   
∴EPN≌GQN AAS
![](<../../qs_image_DB/专题1-1_一网打尽全等三角形模型_·十个模型（解析版）/358d25f351cb40b11bf281fd3c51e0484ed7b03184823590d32845f0d9aea3f0.jpg>)  
图3
【淘宝店铺：向阳百分百】 $\cdot \ N P = N Q$ ，
∵ $\angle C A G = 9 0 ^ { \circ }$ ，  
$\therefore \angle Q A G + \angle C A M = 1 8 0 ^ { \circ } - 9 0 ^ { \circ } = 9 0 ^ { \circ }$   
∵ $A M \perp B C$ ，  
$\angle A C M + \angle C A M = 9 0 ^ { \circ }$   
$\angle A C M = \angle Q A G$ ，  
在 $\triangle Q A G$ 和 $\triangle M C A$ 中，  
$\left\{ \begin{array} { l } { \angle Q A G = \angle M C A } \\ { \angle A Q G = \angle C M A , } \\ { A G = A C } \end{array} \right.$   
∴QAG≌MCAAAS ，  
∴ AQ  CM  1，  
∴ PQ  AP  AQ  4 1  3 ，  
∴ NP  NQ 3 2 ,3 5  
∴ 1AN  AQ  NQ  2 2  
$\therefore S _ { \scriptscriptstyle \mathrm { \partial } A E G } = \frac { 1 } { 2 } A N \cdot E P + \frac { 1 } { 2 } \cdot A N \cdot G Q = \frac { 1 } { 2 } \times \frac { 5 } { 2 } \times \left( 3 + 3 \right) = \frac { 1 5 } { 2 } ,$
