【详解】（1）解：法一：

![](<../../qs_image_DB/专题1-1_一网打尽全等三角形模型_·十个模型（解析版）/89aef86c94dde7f6f6e7f1a6b2ea60e419f6306e7826db1cb07867ee38f97e8f.jpg>)

如图：延长 $A B$ 交 $C F$ 于点 $D$ ，  
∵等腰 $\mathrm { R t } _ { \Delta A B C , \mathrm { R t } _ { \Delta } C E F }$ 有公共顶点 $C$ ， $\angle A B C = \angle C E F = 9 0 ^ { \circ }$ ，$\angle E C D = 4 5 ^ { \circ } \angle C B D = 9 0 ^ { \circ } \angle A B = B C$   
∴ $\cdot \angle B D C = 9 0 ^ { \circ } - 4 5 ^ { \circ } = 4 5 ^ { \circ } = \angle B C D$   
∴ $A B = B C = B D$ ，  
∴点 $B$ 为线段 $A D$ 的中点，  
又∵点 $M$ 为线段 $A F$ 的中点，  
∴ BM 为 $\triangle A D F$ 的中位线，  
$B M / / C F$ ；

法二：

![](<../../qs_image_DB/专题1-1_一网打尽全等三角形模型_·十个模型（解析版）/e094e59f4a89a935cb2ac1d1f3abcc172a224b688151db59c6a3dc0387eb601b.jpg>)

如图，延长 $B M$ 交 $E F$ 于 $D$ ，  
∵ $\angle A B C = \angle C E F = 9 0 ^ { \circ } .$ ，  
$A B \bot C E , E F \bot C E$ ，  
$\therefore A B / / E F$ ，  
$\therefore \angle B A M = \angle D F M$ ，  
∵ $M$ 是 $A F$ 的中点，  
$A M = M F$ ，  
在 $\triangle A B M$ 和 $\triangle F D M$ 中，  
$\left\{ \begin{array} { c } { { \angle B A M = \angle D F M } } \\ { { A M = F M } } \\ { { \angle A M B = \angle F M D } } \end{array} \right. ,$   
$\therefore \Delta A B M \cong \Delta F D M \left( \mathrm { A S A } \right) ,$   
$A B = D F$ ，  
$B E = C E - B C , D E = E F - D F$ ，  
$\mathbf { \partial } \cdot \mathbf { \partial } B E = D E$ ，  
∴ $\mathbf { \nabla } \cdot \triangle B D E$ 是等腰直角三角形，  
∴ $\angle E B M = 4 5 ^ { \circ }$ ，  
∵在等腰直角 $\triangle C E F$ 中， $\angle E C F = 4 5 ^ { \circ }$ ，∴ $\angle E B M = \angle E C F$ ，  
∴ $M B / / C F$ ；  
（2）法一：  
如图，延长 $A B$ 交 $C E$ 于点 $\cdot$ ，连接 $D F$ ，则： $\angle C B D = 9 0 ^ { \circ }$ ，  
∵ $\angle B C E = 4 5 ^ { \circ }$ ，  
∴ $\angle B D C = 9 0 ^ { \circ } - 4 5 ^ { \circ } = 4 5 ^ { \circ } = \angle B C D$ ，  
$B D = B C$ ，  
∵ ${ \triangle A B C }$ 为等腰直角三角形，$A B = B C$ ，  
$A B = B C = B D A C = C D$ ，  
∴点 $B$ 为 $A D$ 中点，又点 $\cdot$ 为 $A F$ 中点，  
$B M = { \frac { 1 } { 2 } } D F$   
延长 $F E$ 与 $C B$ 交于点 $\cdot$ ，连接 $_ { A G }$ ，  
同法可得： $C E = E F = E G$ ， $C F = C G$ ，  
∴点 $\cdot$ 为 $F G$ 中点，又点 $\cdot$ 为 $A F$ 中点，  
$\therefore M E = { \frac { 1 } { 2 } } A G .$   
在 $\triangle A C G$ 与 $\triangle D C F$ 中，  
$\left\{ \begin{array} { c } { { A C = C D } } \\ { { \angle A C G = \angle D C F = 4 5 ^ { \circ } , } } \\ { { C G = C F } } \end{array} \right.$   
$\scriptstyle \triangle A C G \cong \triangle D C F ( \mathrm { S A S } )$ ，  
$D F = A G$ ，  
$B M = M E$ ．

![](<../../qs_image_DB/专题1-1_一网打尽全等三角形模型_·十个模型（解析版）/f3cffefaf562abf5a45bddce5ca9b9bfdd9265884ab80ec6b40bfe75f4b1faa4.jpg>)

法二：

![](<../../qs_image_DB/专题1-1_一网打尽全等三角形模型_·十个模型（解析版）/f04c8065149521a448474dbb7ea0a44643b603a00a4fbede341aec550a613c62.jpg>)

如图，延长 BM 交 $C F$ 于 $D$ ，连接 $B E$ 、 $D E$ ，  
∵ ${ \triangle A B C }$ 为等腰直角三角形， $\triangle E C F$ 为等腰直角三角形，  
$\angle A C B = \angle B A C = 4 5 ^ { \circ }$ ， $\angle E C F = 4 5 ^ { \circ }$ ，  
∵ $\angle B C E = 4 5 ^ { \circ }$ ，  
∴ $. \angle A C D = 4 5 ^ { \circ } \times 2 + 4 5 ^ { \circ } = 1 3 5 ^ { \circ }$ ，  
$\angle B A C + \angle A C F = 4 5 ^ { \circ } + 1 3 5 ^ { \circ } = 1 8 0 ^ { \circ }$   
$\therefore A B / / C F$ ，  
$\angle B A M = \angle D F M$ ，  
∵ $M$ 是 $A F$ 的中点，  
$\mathbf { A M } = \mathbf { F M }$ ，  
在 $\triangle A B M$ 和 $\triangle F D M$ 中，  
$\left\{ \begin{array} { c } { { \angle B A M = \angle D F M } } \\ { { A M = F M } } \\ { { \angle A M B = \angle F M D } } \end{array} \right. ,$   
$\therefore \Delta A B M \cong \Delta F D M \left( \mathrm { A S A } \right) ,$ ，  
$\therefore A B = D F , B M = D M \ ,$ ，  
$A B = B C = D F$ ，  
在 $\triangle B C E$ 和 $\triangle D F E$ 中，  
$\left\{ \begin{array} { c } { { B C = D F } } \\ { { \angle B C E = \angle D F E = 4 5 ^ { \circ } , } } \\ { { C E = F E } } \end{array} \right.$   
$\therefore \Delta B C E \cong \Delta D F E \left( \mathrm { S A S } \right) ,$   
$B E = D E \angle B E C = \angle D E F$ ，  
$\angle B E D = \angle B E C + \angle C E D = \angle D E F + \angle C E D = \angle C E F = 9 0 ^ { \circ }$ ，  
$\triangle B D E$ 是等腰直角三角形，  
又∵ $B M = D M$ ，  
$\therefore B M = M E = { \frac { 1 } { 2 } } B D ,$   
∴ $\mathbf { \partial } _ { \cdot } B M = M E$
