【详解】延长 $A C$ 至 $D$ ，使得 $A D = B D$ ，连接 $B D$ ，如图

![](<../../qs_image_DB/专题1-1_一网打尽全等三角形模型_·十个模型（解析版）/d9a2c707dbb3601c232c3e860dd9b4ecfcef8b73ed75f1b23c8811472e0306eb.jpg>)

∵ $\angle C A B = 6 0 ^ { \circ }$   
∴ $\triangle A B D$ 为等边三角形  
∵ $B C$ 绕着点 $B$ 逆时针旋转 $6 0 ^ { \circ }$ 得到 $B C$ '  
∴ $\triangle B C C ^ { \prime }$ 为等边三角形  
$\therefore B C = B C ^ { \prime } , \angle C B C ^ { \prime } = 6 0 ^ { \circ }$   
$\therefore \angle D B A - \angle A B C = \angle C B C ^ { \prime } - \angle A B C$   
即 $\angle D B C = \angle A B C ^ { \prime }$ '  
在 $\triangle D B C$ 和 $\triangle A B C ^ { \prime }$ 中  
$\left\{ \begin{array} { c } { { D B = D B } } \\ { { \angle D B C = \angle A B C ^ { \prime } } } \\ { { B C = B C ^ { \prime } } } \end{array} \right.$   
$\therefore \Delta D B C \cong \Delta A B C ^ { \prime }$ （ SAS ）  
$\therefore S _ { \scriptscriptstyle \triangle D B C } = S _ { \scriptscriptstyle \triangle A B C } ,$   
过点 $B$ 作 $B E \bot A D$ 于点 $E$   
$\therefore \angle D B E = 9 0 ^ { \circ } - \angle D = 3 0 ^ { \circ }$   
$\therefore D E = { \frac { 1 } { 2 } } B D = { \frac { 1 } { 2 } } A B = 5$   
${ \begin{array} { c } { \displaystyle ^ { \angle } } \\ { \displaystyle B E = { \sqrt { B D ^ { 2 } - D E ^ { 2 } } } = 5 { \sqrt { 3 } } \quad D C = A D - A C = 1 0 - 6 = 4 } \\ { \displaystyle S _ { _ { \Delta D B C } } = { \frac { 1 } { 2 } } \cdot D C \cdot B E = { \frac { 1 } { 2 } } \times 4 \times 5 { \sqrt { 3 } } = 1 0 { \sqrt { 3 } } } \\ { \displaystyle S _ { _ { \Delta A B C } } = 1 0 { \sqrt { 3 } } } \end{array} }$
