【详解】解：∵ $\angle B A D = 6 0 ^ { \circ }$ ， $A B = A D$ ，将 $\triangle A C D$ 绕点 A 逆时针旋转 $6 0 ^ { \circ }$ ，得 $\triangle A B C _ { 1 }$ ，如图所示，

![](<../../qs_image_DB/专题1-1_一网打尽全等三角形模型_·十个模型（解析版）/819c58db27fd1980281c697efc00e279890465682c87840eccdc7d97d935565a.jpg>)

∴ $\angle A B C _ { 1 } = \angle D$ ， $A C = A C _ { 1 }$ ，  
∴ $\angle C A C _ { 1 } = 6 0 ^ { \circ }$ ，  
∵ $\angle A B C + \angle D = 1 8 0 ^ { \circ }$ ，则 $\angle A B C + \angle A B C _ { 1 } = 1 8 0 ^ { \circ }$   
∴点 $C _ { 1 }$ 在 $C B$ 的延长线上，且 $A C _ { 1 } = A C$ ， $\angle C A C _ { 1 } = 6 0 ^ { \circ }$ ，  
∴ $\triangle A C C _ { 1 }$ 是等边三角形，过点 A 作 $A E \perp B C _ { 1 }$ 于 $E$ ， $A C = 2$ ，  
∴ $C C _ { 1 } = 2$ ， $A E = { \sqrt { 3 } }$ ，  
$\therefore S _ { \triangle A C C _ { 1 } = } = \frac { 1 } { 2 } C C _ { 1 } \bullet A E = \frac { 1 } { 2 } \times 2 \times \sqrt { 3 } = \sqrt { 3 } \ ,$ ，  
$\therefore S _ { \substack { _ { [ \mathbb { H } \ni \pmb { \mathscr { H } } \mathscr { H } \ A B C D } } } = S _ { \triangle A C C _ { 1 } } = \frac { \sqrt { 3 } } { 4 } A C ^ { 2 } = \frac { \sqrt { 3 } } { 4 } \times 2 ^ { 2 } = \sqrt { 3 }$
