例49 请解答以下各题：
∴ $O E = 5 a$ ，   
$\therefore \sin E = \frac { O C } { O E } = \frac { 3 } { 5 } , \cos E = \frac { 4 } { 5 }$ 即 $\frac { 3 } { 5 } = \frac { O C } { O C + 4 }$   
解得： $O C { = } 6$ ，   
$O C \bot D E$ ，   
$\therefore \angle B C E + \angle O C B = 9 0 ^ { \circ }$   
∵ $O C = O B$   
∴ $. \angle O C B = \angle O B C$ ，   
$\therefore \angle B C E + \angle O B C = 9 0 ^ { \circ }$ ，   
∵ $A B$ 是直径，   
∴ $\angle A C B = 9 0 ^ { \circ }$ ，   
$\angle C A B + \angle A B C = 9 0 ^ { \circ }$   
∴ $\angle B C E = \angle C A E$ ，   
又 $\angle E = \angle E$ ，   
$\triangle B C E \sim \triangle C A E$ ，   
$\frac { C E } { A E } = \frac { B E } { C E } \frac { C B } { C A } = \frac { C E } { A E }$   
$\therefore C E ^ { 2 } = B E \times A E$ ，   
$C E ^ { 2 } = 4 \times { \left( { 4 + 1 2 } \right) } = 6 4$ ，   
解得： $C E = 8$ ，   
${ \frac { C B } { C A } } = { \frac { C E } { A E } } = { \frac { 8 } { 1 2 + 4 } } = { \frac { 1 } { 2 } }$   
∴ tan $\angle C A B = \frac { B C } { A C } = \frac { 1 } { 2 }$   
∵ $A B$ 是 $_ { \odot O }$ 的直径，   
$B F \bot A F$ ，   
$\therefore D E \bot A D$ ，   
∴ DC ∥ FB   
∴? FBA $? E$ ，   
∴ tan $\angle F B A = \tan \angle E$ ，   
$\scriptstyle \cdot { \frac { A F } { F B } } = { \frac { O C } { C E } } = { \frac { 6 } { 8 } } = { \frac { 3 } { 4 } } ,$   
设 $A F = 3 k$ ，则 $F B = 4 k$ ，   
∴ $A B = 5 k$ ，   
∵ $A B = 1 2$ ,   
$\therefore k = { \frac { 1 2 } { 5 } } ,$ ,   
$\therefore A F = \frac { 3 6 } { 5 }$ $F G \bot A B$ ，   
∴ $\angle A F G = 9 0 ^ { \circ } - \angle G F B = \angle F B A = \angle E$   
$\begin{array} { l } { { \displaystyle { \therefore F G = A F \times \cos E = \frac { 4 } { 5 } A F = \frac { 4 } { 5 } \times \frac { 3 6 } { 5 } = \frac { 1 4 4 } { 2 5 } , } } } \\ { { \displaystyle { \therefore A G = \frac { 3 } { 5 } A F = \frac { 1 0 8 } { 2 5 } } , } } \end{array}$   
∵ $\tan \angle C A B = \tan \angle H A G = \frac { 1 } { 2 } = \frac { H G } { A G }$
![](<../../qs_image_DB/专题3-6__圆的综合（27类题型）（解析版）/965f3846c69458d0c70c722d4d961cad530d254b637e70eb948d12dc1b330958.jpg>)
$H G = { \frac { 1 } { 2 } } A G = { \frac { 5 4 } { 2 5 } }$ $\therefore F H = F G - H G = \frac { 1 4 4 } { 2 5 } - \frac { 5 4 } { 2 5 } = \frac { 9 0 } { 2 5 } = \frac { 1 8 } { 5 } .$
