例89 请解答以下各题：
![](<../../qs_image_DB/专题3-6__圆的综合（27类题型）（解析版）/9c745a8c6cb775935ae92af6634f53e73d2c7c4271c1894d555f2e2f1dc178ef.jpg>)
∵ $\cdot$ 为正方形中心，  
∴ $\cdot \angle O A B = \angle O A D = \angle O D A = 4 5 ^ { \circ } ,$ ， $\angle A O D = 9 0 ^ { \circ }$ ，而 $\angle B A E = 3 0 ^ { \circ }$ ，  
∴ $\angle O A E = 7 5 ^ { \circ }$ ， $\angle E A D = 3 0 ^ { \circ } + 9 0 ^ { \circ } = 1 2 0 ^ { \circ }$   
∵ $\angle E A G = 9 0 ^ { \circ }$ ，  
∴ $\angle F A D = 1 2 0 ^ { \circ } - 9 0 ^ { \circ } = 3 0 ^ { \circ }$ ，  
$\therefore A F = 2 x , A K = \sqrt { 3 } x ,$ ，$\angle A E D = \frac { 1 } { 2 } \angle A O D = 4 5 ^ { \circ }$   
$\therefore \angle A F D = \angle A E D + \angle E A F = 4 5 ^ { \circ } + 9 0 ^ { \circ } = 1 3 5 ^ { \circ }$   
$\angle A D F = 1 8 0 ^ { \circ } - 3 0 ^ { \circ } - 1 3 5 ^ { \circ } = 1 5 ^ { \circ } \qquad Q F = Q D$ ，  
∴ $\angle Q F D = \angle Q D F = 1 5 ^ { \circ }$ ，  
∴ $\angle K Q F = 3 0 ^ { \circ }$ ，  
$F Q = 2 x = Q D \quad Q K = \sqrt { 3 } x$ ，  
而正方形的边长 $A B = 2 = A D$ ，  
$\therefore 2 { \sqrt { 3 } } x + 2 x = 2$ ，  
解得： $x = { \frac { { \sqrt { 3 } } - 1 } { 2 } }$   
$\begin{array} { l } { { S _ { \scriptscriptstyle { A d F D } } = \displaystyle \frac { 1 } { 2 } { \cal A } D { \cdot } F K = \displaystyle \frac { 1 } { 2 } { \times } 2 { \times } \displaystyle \frac { \sqrt { 3 } - 1 } { 2 } = \displaystyle \frac { \sqrt { 3 } - 1 } { 2 } } } \\ { { \ A D = 2 \quad \it { A O D } = 9 0 \mathrm { ^ { o } } \quad \it { O A } = O D } } \\ { { \ O A = O D = A D { \times } \displaystyle \frac { \sqrt { 2 } } { 2 } = \sqrt { 2 } } } \\ { { \ S _ { \scriptscriptstyle { A d D } } = \displaystyle \frac { 1 } { 2 } { \times } \sqrt { 2 } { \times } \sqrt { 2 } = 1 } } \end{array}$   
而 $S _ { \scriptscriptstyle \boxplus \boxplus \boxplus } S _ { \scriptscriptstyle \boxplus \boxed { \ell } } = \frac { 9 0 \pi \times \left( \sqrt { 2 } \right) ^ { 2 } } { 3 6 0 } { = } \frac { 1 } { 2 } \pi$   
$\therefore S _ { \scriptscriptstyle  { \boxplus \ncong \atop 2 } } = \frac { 1 } { 2 } \pi - 1 + \frac { \sqrt { 3 } - 1 } { 2 } = \frac { \pi + \sqrt { 3 } - 3 } { 2 } \ : .$
