【详解】（1）证明：如图所示，过点 $F$ 作 $F H \bot A C , F G \bot A B$ ，垂足分别为 $H , G$ ，

![](<../../qs_image_DB/专题3-6__圆的综合（27类题型）（解析版）/40c2ea25d9be6a2bde830f534cb82a0f007b36cd1b3ef8a26b20b3f52784c304.jpg>)

∵点 $E$ 是 ${ \triangle A B C }$ 的内心，∴ $A D$ 是 $\angle B A C$ 的角平分线，$F H \bot A C , F G \bot A B$ ，∴ $F G = F H$ ，

$S _ { \scriptscriptstyle \Delta A B F } = \frac { 1 } { 2 } A B \cdot F G , S _ { \scriptscriptstyle \Delta A C F } = \frac { 1 } { 2 } A C \cdot F H$ $S _ { \triangle A B F } : S _ { \triangle A C F } = A B : A C$ ； （2）证明：如图所示，过点 $\cdot$ 作 $A M \perp B C$ 于点 $M$ ,

$$
\textcircled { \scriptsize { 1 } } \textcircled { \scriptsize { 1 } } \textcircled { \scriptsize { 1 } } \textcircled { \scriptsize { 1 } } \textcircled { \scriptsize { 2 } } \textcircled { \scriptsize { 1 } } \textcircled { \scriptsize { 2 } } \textcircled { \scriptsize { 1 } } \textcircled { \scriptsize { 2 } } \textcircled { \scriptsize { 1 } } \textcircled { \scriptsize { 2 } } \textcircled { \scriptsize { 1 } } \textcircled { \scriptsize { 2 } } \textcircled { \scriptsize { 1 } } \textcircled { \scriptsize { 2 } } \textcircled { \scriptsize { 1 } } \textcircled { \scriptsize { 2 } } \textcircled { \scriptsize { 1 } } \textcircled { \scriptsize { 2 } } \textcircled { \scriptsize { 2 } } \textcircled { \scriptsize { 1 } } \textcircled { \scriptsize { 2 } } \textcircled { \scriptsize { 2 } } \textcircled { \scriptsize { 1 } } 
$$

$\because S _ { _ { \Delta A B F } } = \frac { 1 } { 2 } B F \cdot A M , S _ { _ { \Delta A C F } } = \frac { 1 } { 2 } F C \cdot A M \ ,$ ，  
$\therefore S _ { \triangle A B F } : S _ { \triangle A C F } = B F : F C \ ,$   
由（1）可得 $S _ { \triangle A B F } : S _ { \triangle A C F } = A B : A C$ ，  
$\therefore A B : A C = B F : C F :$   
（3）证明：连接 $D B , D C$ ，

$$
\underset { \ b { p } } { \overset { \displaystyle \bigwedge } { } }
$$

$\widehat { A B } = \widehat { A B } , \widehat { D C } = \widehat { D C }$   
$\therefore \angle A C F = \angle B D F , \angle F A C = \angle F B D$   
∴BFD∽AFC  
${ \frac { B F } { A F } } { = } { \frac { D F } { C F } }$ ,  
$\therefore B F \cdot C F = A F \cdot D F$   
A C  AC ，  
∴ $. \angle F B A = \angle A D C$ ，  
又 $\angle B A D = \angle D A C$ ，  
$\triangle A B F \sim \triangle A D C$ ，  
$\cdot \frac { A B } { A D } { = } \frac { A F } { A C }$ ,  
$A B \cdot A C = A D \cdot A F$ ；  
$\therefore A B \cdot A C = \left( A F + D F \right) \cdot A F = A F ^ { 2 } + A F \cdot D F \ ,$ $\therefore A F ^ { 2 } = A B \cdot A C - B F \cdot C F ,$ ，  
（4）解：如图所示，连接 $B E$ ，  
