【答案】A

【分析】如图，过 $C$ 作 $C H \bot A O$ 于 $H$ ，证明 $\angle C O D = \angle B O E = \angle C A O$ ， 由 $\frac { S _ { 1 } } { S _ { 2 } } = \frac { 2 } { 3 }$ 即 $\frac { \frac { 1 } { 2 } O A \bullet C H } { \frac { 1 } { 2 } O B \bullet B E } = \frac { 2 } { 3 } ,$ 可得 ${ \frac { C H } { B E } } { = } { \frac { 2 } { 3 } }$ ， 证明 tan $\angle A = \tan \angle B O E$ ，可得 $\frac { C H } { B E } { = } \frac { A H } { O B } { = } \frac { 2 } { 3 }$ ， 设 $A H = 2 m$ ，则 $B O = 3 m = A O = C O$ ，可得 $O H = 3 m - 2 m = m$ ， $C H = \sqrt { 9 m ^ { 2 } - m ^ { 2 } } = 2 \sqrt { 2 } m$ ，再利用正切的定义可得答案．
