例15 请解答以下各题：
 A1，0 ， $\cdot \begin{array} { l } { { \left\{ - k + b = 0 \right. } }  \\ { { \left. k m + b = - m ^ { 2 } + 2 m + 3 \right.} } \end{array} $ 解得： $\begin{array} { c } { { \{ k = - ( m - 3 )  } } \\ { {  b = - ( m - 3 ) } ^ { , } } \end{array}$ ，  
直线 $A P$ 的解析式为 $y = - ( m - 3 ) x - ( m - 3 )$ ，当 $x = 0$ 时， $y = - ( m - 3 ) = 3 - m$ ，  
$\therefore \left( 0 , 3 - m \right) \quad \therefore O D = 3 - m \quad \therefore C F = O D = 3 - m$ ，  
在抛物线 $y = - x ^ { 2 } + 2 x + 3$ 中，当 $x = 0$ 时， $y = 3$ ，C 0，3， $O C = 3$ ，  
$\therefore D F = O C - O D - C F = 3 - \left( 3 - m \right) - \left( 3 - m \right) = 2 m - 3$ ，  
设点 $E$ 的坐标 $\begin{array} { r l r l r l } { \big ( t , - \big ( m - 3 \big ) t - \big ( m - 3 \big ) \big ) } & { { } \because A \big ( - 1 , 0 \big ) } & { } & { { } B \big ( 3 , 0 \big ) } & { } & { { } \colon A B = 4 } & { } & { { } \colon S _ { \triangle A F E } = S _ { \triangle A B E } } \end{array}$ ，
$\therefore \frac { 1 } { 2 } D F \cdot \left( x _ { 4 } - x _ { E } \right) = \frac { 1 } { 2 } A B \cdot y _ { E } , \therefore \frac { 1 } { 2 } \times \left( 2 m - 3 \right) \times \left( t + 1 \right) = \frac { 1 } { 2 } \times 4 \times \left[ - \left( m - 3 \right) t - \left( m - 3 \right) \right] ,$ 解得： $m = \frac { 5 } { 2 }$ ， 点 $P$ 的坐标为 $\left( \frac { 5 } { 2 } , \frac { 7 } { 4 } \right)$ ， $\therefore S _ { \scriptscriptstyle \triangle P A B } = \frac { 1 } { 2 } A B \times y _ { \scriptscriptstyle P } = \frac { 1 } { 2 } \times 4 \times \frac { 7 } { 4 } = \frac { 7 } { 2 } .$
