【答案】(1)6(2)见解析

【思路点拨】（1）把 $C \left( 1 , 3 \right)$ 代入 $y = a x ^ { 2 } - 3$ ，得 $3 = a - 3$ ，即可求出 $a$ 的值；（2）设直线 $\begin{array} { r l } { C A } & { { } y = k x + b } \end{array}$ 与抛物线 $y = a x ^ { 2 } - 3$ 交于 $C \_ { \mathrm { ~ \tiny ~ A ~ } }$ 两点，联立 $\left\{ \begin{array} { l l } { y = a x ^ { 2 } - 3 } \\ { y = k x + b } \end{array} \right.$ 得出 $x _ { _ { A } } \cdot x _ { _ { C } } = { \frac { - b - 3 } { a } }$ ,设直线 $B C$ 为： $y = k _ { 1 } x + b _ { 1 }$ ，联立 $\left\{ { \begin{array} { l } { y = k _ { 1 } x + b _ { 1 } } \\ { y = a x ^ { 2 } - 3 } \end{array} } \right.$ ，得出 $x _ { _ B } \cdot x _ { _ c } = { \frac { - b _ { _ 1 } - 3 } { a } }$ ，再由 $x _ { \mathrm { \mathcal { A } } } + x _ { B } = 0$ 得出 $- b - b _ { 1 } = 6$ ，最后再根据 $O E - O D = - b _ { 1 } - b = 6$ 即可得到答案．
