【详解】（1）解：令 $y = 0$ 得 $x ^ { 2 } - 2 x - 3 = 0$ ，  
解得 $x _ { 1 } = - 1$ ， $x _ { 2 } = 3$ ，  
令 $x = 0$ 得 $y = - 3$ ，  
∴点 $\cdot$ ， $B$ ， $\cdot$ 的坐标分别是 $\left( - 1 , 0 \right) , \left( 3 , 0 \right) , \left( 0 , - 3 \right)$ ；  
（2）解：由平移得 ${ \cal C } _ { _ 2 } \mathrm { ~  ~ \psi ~ } y = x ^ { 2 }$ ，  
设点 $E { \Big ( } e , e ^ { 2 } { \Big ) }$ ， $F \left( f , f ^ { 2 } \right)$ ， $M \left( m , m ^ { 2 } \right)$ ， $P E$ 的解析式为 $y = k x + k$ ，  
联立 $\scriptstyle { \left\{ \begin{array} { l l } { y = k x + k } \\ { y = x ^ { 2 } } \end{array} \right. }$ ，得 $x ^ { 2 } - k x - k = 0$ ，  
$ e + f = k e f = - k$ ，  
$\therefore e + f + e f = 0 . \textcircled { \scriptsize { 1 } }$   
∵ $E M$ 与直线 $y = - 2 x$ 平行，  
∴设直线 $E M$ 的解析式为 $y = - 2 x + b$ ，  
联立 $\left\{ \begin{array} { c } { y = - 2 x + b } \\ { y = x ^ { 2 } } \end{array} \right.$ , 得 $x ^ { 2 } + 2 x - b = 0$ ，  
∴ $e + m = - 2$ ， $\cdot$   
联立 $\textcircled{1} \textcircled{2}$ 得 $- m f = \left( m + f \right) + 2$   
设直线 $F M$ 的解析式为 $y = n x + t$   
$\cdot \left\{ { { m } ^ { 2 } } = n m + t \right.$ 解得 ${ \begin{array} { c } { \left( n = m + f \right. } \\ { \left. t = - m f \right. } \end{array} } ,$   
∴直线 $F M$ 的解析式为 $y = ( m + f ) x - m f = ( m + f ) x + ( m + f ) + 2$ ，  
当 $x { = } - 1$ 时， $y = 2$ ，故直线 $F M$ 经过定点 $\left( - 1 , 2 \right)$

# 2024 届·福建厦门市第九中学期中
