【答案】 $( 1 ) y = - x ^ { 2 } + 2 x + 3$ (2)见解析

【思路点拨】（1）利用待定系数法即可求得答案；

（2）先求得平移后的抛物线 $C _ { 2 }$ 的解析式为： $y = - x ^ { 2 } + 4$ ，设 $M ( m , - m ^ { 2 } + 4 )$ ， $N ( n , - n ^ { 2 } + 4 )$ ，则直 线 MN的解析式为 $y = - ( m + n ) x + m n + 4$ ，由直线MN 经过定点 $F ( 0 . 5 , 1 )$ ，可得 $m + n = 2 m n + 6$ ，再由直线$y = - x + b$ 经 过 点 $M ( m , - m ^ { 2 } + 4 )$ ， 可 得 直 线 $M P$ 的 解 析 式 为 $y = - x - m ^ { 2 } + m + 4$ ， 进 而 求 得$P ( 1 - m , - m ^ { 2 } + 2 m + 3 )$ ，再运用待定系数法求得直线 $P N$ 的解析式为 $y = ( m - n - 1 ) x - { \frac { 1 } { 2 } } ( m - n ) + 7$ ，当 $x = \frac { 1 } { 2 }$ 时， $y = { \frac { 1 } { 2 } } ( m - n - 1 ) - { \frac { 1 } { 2 } } ( m - n ) + 7 = { \frac { 1 3 } { 2 } }$ 即直线 $N P$ 必过 定点 $( \frac { 1 } { 2 } , ~ \frac { 1 3 } { 2 } )$
