【详解】（1）解：抛物线 $y = a x ^ { 2 } - 2 a x + c$ 经过点 $A ( - 1 , 0 )$ ， $C ( 2 , 3 )$ ，$\cdot \left\{ { a + 2 a + c = 0 \atop 4 a - 4 a + c = 3 } \right.$ 解得： $\scriptstyle { \left\{ \begin{array} { l l } { a = - 1 } \\ { c = 3 } \end{array} \right. }$ , 抛物线 $C _ { 1 }$ 的解 析式 为 $y = - x ^ { 2 } + 2 x + 3$ ；

（2）证明：如图 2，抛物线 $C _ { 1 } : y = - x ^ { 2 } + 2 x + 3 = - ( x - 1 ) ^ { 2 } + 4$ ，将抛物线 $C _ { 1 }$ 沿 $x$ 轴平移得 $C _ { 2 }$ ，使 $C _ { 2 }$ 的顶点落在 $y$ 轴上，抛物线 $C _ { 2 }$ 的解析式为： $y = - x ^ { 2 } + 4$ ，

![](<../../qs_image_DB/专题3-1_二次函数中的10类定值、定点问题（解析版）/eb71a95b0c7a0d381e4140d64ba4c06959dcac03fdee6e55961b6d12eb4ecfaa.jpg>)  
图2

设 $M ( m , - m ^ { 2 } + 4 )$ ， $N ( n , - n ^ { 2 } + 4 )$ ，  
则直线 $M N$ 的解析式为 $y = - ( m + n ) x + m n + 4$ ，  
直线MN 经过定点 $F ( 0 . 5 , 1 )$ ，  
$\therefore 1 = - { \frac { 1 } { 2 } } ( m + n ) + m n + 4$ ，  
$\cdot m + n = 2 m n + 6$ ，  
直线 $y = - x + b$ 经过点 $M ( m , - m ^ { 2 } + 4 )$ ，  
$\cdot - m ^ { 2 } + 4 = - x + b$ ，  
解得： $b = - m ^ { 2 } + m + 4$ ，  
直线 $M P$ 的解析式为 $y = - x - m ^ { 2 } + m + 4$ ，  
由 $- x ^ { 2 } + 4 = - x - m ^ { 2 } + + m + 4$ ，  
解得： $x = m$ 或 $x = 1 - m$ ，  
$\therefore P ( 1 - m , - m ^ { 2 } + 2 m + 3 )$ ，  
设直线 $P N$ 的解析式为 $y = k ^ { \prime } x + b ^ { \prime }$ ，把 $P ( 1 - m , - m ^ { 2 } + 2 m + 3 )$ ， $N ( n , - n ^ { 2 } + 4 )$ 代入，  
得 $\left\{ \begin{array} { l } { { ( 1 - m ) k ^ { \prime } + b ^ { \prime } = - m ^ { 2 } + 2 m + 3 } } \\ { { n k ^ { \prime } + b ^ { \prime } = - n ^ { 2 } + 4 } } \end{array} \right.$   
解得： $\left\{ \begin{array} { l l } { \displaystyle k ^ { \prime } = m - n - 1 } \\ { \displaystyle b ^ { \prime } = - m n + n + 4 } \end{array} , \right. \because m + n = 2 m n + 6 \ , ~ \therefore m n = \frac { m + n } { 2 } - 3 \ ,$   
$\therefore b ^ { \prime } = - { \frac { m + n } { 2 } } + 3 + n + 4 = - { \frac { 1 } { 2 } } ( m - n ) + 7 \ ,$   
直线 $P N$ 的解析式为 $y = ( m - n - 1 ) x - { \frac { 1 } { 2 } } ( m - n ) + 7$ ，$x = \frac { 1 } { 2 }$ 时， $y = \frac 1 2 ( m - n - 1 ) - \frac 1 2 ( m - n ) + 7 = \frac { 1 3 } 2 ,$   
直线 $N P$ 必过定点 $( { \frac { 1 } { 2 } } \quad { \frac { 1 3 } { 2 } } )$

# 2023 广东省梅州市九年级下期中
