【答案】 $( 1 ) y \ = \ { \frac { 1 } { 4 } } \ x ^ { 2 }$

(2)见解析

【思路点拨】（1）根据顶点是原点，设函数解析式为 $y = a x ^ { 2 }$ ，将2,1代入求得 $a$ 的值即可得到二次函数的表达式；

（2）联立 $\left\{ \begin{array} { l l } { \displaystyle y = k x - 2 k } \\ { \displaystyle y = \frac { 1 } { 4 } x ^ { 2 } } \end{array} \right.$ 得到 $x ^ { 2 } - 4 k x + 8 k = 0$ ，则 $\left\{ { \begin{array} { l } { \displaystyle x _ { _ { E } } + x _ { _ { D } } = 4 k } } \\ { \displaystyle x _ { _ { E } } \cdot x _ { _ { D } } = 8 k } \end{array}  \right. \textcircled { 1 }$ ，联立 $\left\{ \begin{array} { l l } { y = x + b } \\ { \displaystyle y = \frac { 1 } { 4 } x ^ { 2 } } \end{array} \right.$ 得到 ${ \frac { 1 } { 4 } } x ^ { 2 } - x - b = 0$ ，则 $\left\{ { \begin{array} { l } { x _ { _ { D } } + x _ { _ { F } } = 4 } \\ { x _ { _ { D } } \cdot x _ { _ { F } } = - 4 b } \end{array} } \right.$ ，令 $l _ { \scriptscriptstyle E F } \colon \ y = m x + n$ ， 联 立 $\left\{ \begin{array} { l l } { \displaystyle y = m x + n } \\ { \displaystyle y = \frac { 1 } { 4 } x ^ { 2 } } \end{array} \right.$ 得到 $\begin{array} { c c } { { \displaystyle { \frac { 1 } { 4 } } x ^ { 2 } - m x - n = 0 \quad } } & { { \left\{ x _ { { \cal E } } + x _ { { \cal F } } = 4 m \begin{array} { l } { { } } \\ { { y _ { \cal E } \cdot x _ { { \cal F } } = - 4 n } } \end{array} \right. } } \end{array}$ 整理得到 $n = - 2 m + 2$ ，得到 $\begin{array} { r l } { l _ { E F } } & { { } \ y = m x - 2 m + 2 = m \left( x - 2 \right) + 2 } \end{array}$ ， 即可证明结论
