【详解】（1）解：∵ $\left( 0 , 0 \right)$ 为顶点，∴设函数解析式为 $y = a x ^ { 2 }$ ，  
将2,1 代入得 $1 = 4 a$ ，∴ $a = { \frac { 1 } { 4 } }$ ∴函数解析式为 $y \ = \ { \frac { 1 } { 4 } } \ x ^ { 2 }$ （2）解：联立 $\left\{ \begin{array} { l } { \displaystyle \boldsymbol { y } = k \boldsymbol { x } - 2 k } \\ { \displaystyle \boldsymbol { y } = \frac { 1 } { 4 } \boldsymbol { x } ^ { 2 } } \end{array} \right. \overset { \ell ^ { \infty } } { \underset { \ell ^ { \infty } } { \longrightarrow } } \boldsymbol { \sharp } \boldsymbol { \sharp } \boldsymbol { \underline { \boldsymbol { x } } } ^ { 2 } - 4 k \boldsymbol { x } + 8 k = 0 \ , ~ \therefore \left\{ \boldsymbol { x } _ { E } + \boldsymbol { x } _ { D } = 4 k \begin{array} { l } { \displaystyle \boldsymbol { \mathcal { D } } , } \\ { \displaystyle \boldsymbol { x } _ { E } \cdot \boldsymbol { x } _ { D } = 8 k } \end{array} \right. \mathbb { O } \left( \frac { 3 } { 2 } , \frac { 2 \pi } { \boldsymbol { \mathcal { D } } _ { E } } \right) = 0 .$   
联立 $\left\{ \begin{array} { l l } { \displaystyle y = x + b } \\ { \displaystyle y = \frac { 1 } { 4 } x ^ { 2 } } \end{array} \right.$ 得到 $\frac { 1 } { 4 } x ^ { 2 } - x - b = 0 , \left\{ { x _ { { D } } + x _ { { F } } = 4 \atop x _ { { D } } \cdot x _ { { F } } = - 4 b } \mathcal { \left( 2 \right) } , \right.$   
令 $l _ { _ { E F } } \quad y = m x + n$ ，联立 $\left\{ \begin{array} { l l } { \displaystyle y = m x + n } \\ { \displaystyle y = \frac { 1 } { 4 } x ^ { 2 } } \end{array} \right.$ 得到 $\begin{array} { c c } { { \displaystyle { \frac { 1 } { 4 } } x ^ { 2 } - m x - n = 0 \quad } } & { { \left\{ x _ { { \cal E } } + x _ { { \cal F } } = 4 m \begin{array} { l } { { } } \\ { { y _ { \cal E } \cdot x _ { { \cal F } } = - 4 n } } \end{array} \right. } } \end{array}$   
由 $\cdot$ 可得 $x _ { F } = 4 - x _ { D }$ 代入 $\textcircled{3}$ 得， $x _ { _ { E } } + 4 - x _ { _ { D } } = 4 m , \quad \cdot \cdot x _ { _ { E } } = x _ { _ { D } } + 4 m - 4 @ ,$ ，  
$x _ { E } \left( 4 - x _ { D } \right) = - 4 n \ , \therefore 4 x _ { E } - x _ { E } \cdot x _ { D } = - 4 n , \therefore 4 x _ { E } - 8 k = - 4 n \textcircled { 6 } ,$   
由∵ $x _ { _ { E } } + x _ { _ { D } } = 4 k \quad x _ { _ { E } } = x _ { _ { D } } + 4 m - 4$   
$\begin{array} { c } { { \therefore 2 x _ { \scriptscriptstyle E } = 4 m - 4 + 4 k , } } \\ { { \therefore 4 x _ { \scriptscriptstyle E } = 8 m - 8 + 8 k \textcircled { 5 } } } \end{array}$   
将 $\textcircled{5}$ 代入 $\cdot$   
$\begin{array} { l } { 8 m - 8 + 8 k - 8 k = - 4 n } \\ { 2 m - 2 = - n } \end{array}$   
即 $n = - 2 m + 2$ ，  
$l _ { E F } \ y = m x - 2 m + 2 = m \left( x - 2 \right) + 2$   
∴ $l _ { E F }$ 过定点 2, 2
# 2023 年湖北省武汉市新观察中考四调
