【详解】（1）解：令 $y = 0$ ， $a x ^ { 2 } + a x - 2 a = 0$ ，$\therefore x _ { 1 } = - 2 x _ { 2 } = 1$ ，  
令 $x = 0$ ，则 $y = - 2 a$ ，  
$\because S _ { \triangle A B C } = { \frac { 1 } { 2 } } A B \cdot O C = { \frac { 3 } { 2 } } ,$   
$\therefore { \frac { 1 } { 2 } } ( 1 + 2 ) ( - 2 a ) = \frac { 3 } { 2 }$   
$\therefore a = - { \frac { 1 } { 2 } }$   
抛物线的解析式为： $\mathbf { y } = - \frac { 1 } { 2 } \mathbf { x } ^ { 2 } - \frac { 1 } { 2 } \mathbf { x } + 1$ ；  
（2）解：设 $P M$ 的解析式为： $y = k _ { 1 } ( x - 2 ) - 2$ ， $P N$ 的解析式为： $y = k _ { 2 } ( x - 2 ) - 2$ ，  
$\begin{array} { r l } & { \therefore M \big ( 0 , - 2 k _ { 1 } - 2 \big ) \quad N \big ( 0 , - 2 k _ { 2 } - 2 \big ) } \\ & { \because O M \cdot O N = 4 } \\ & { \therefore 4 \big ( k _ { 1 } + 1 \big ) \big ( k _ { 2 } + 1 \big ) = - 4 } \\ & { \therefore k _ { 1 } k _ { 2 } + k _ { 1 } + k _ { 2 } + 1 = - 1 } \end{array}$   
联立直线 $P M$ 与抛物线得： $k _ { 1 } ( x - 2 ) - 2 = - \frac { 1 } { 2 } x ^ { 2 } - \frac { 1 } { 2 } x + 1$   
$\therefore x _ { p } \cdot x _ { F } = - 2 \big ( 2 k _ { 1 } + 3 \big ) ,$ ，  
 $x _ { F } = - 2 k _ { 1 } - 3$ 同理： $x _ { { \scriptscriptstyle E } } = - 2 k _ { 2 } - 3$ ，  
联立直线 $E F$ 与抛物线得： $m x + n = - { \frac { 1 } { 2 } } x ^ { 2 } - { \frac { 1 } { 2 } } x + 1$   
$\therefore x _ { _ { E } } + x _ { _ { F } } = - 2 m - 1 , x _ { _ { E } } \cdot x _ { _ { F } } = 2 n - 2 ,$ ，  
即： $- 2 k _ { 1 } - 3 - 2 k _ { 2 } - 3 = - 2 m - 1 , ~ \mathopen { } \mathclose \bgroup \left( - 2 k _ { 1 } - 3 \aftergroup \egroup \right) \mathopen { } \mathclose \bgroup \left( - 2 k _ { 2 } - 3 \aftergroup \egroup \right) = 2 n - 2$ ，  
$\therefore k _ { 1 } + k _ { 2 } = { \frac { 2 m - 5 } { 2 } } k _ { 1 } \cdot k _ { 2 } = { \frac { n - 3 m + 2 } { 2 } }$   
$\therefore n = m - 1$ ，  
$\therefore y = m x + n = m x + m - 1 = m ( x + 1 ) - 1$ ，即：顶点坐标为 $\left( - 1 , - 1 \right)$
