例12 请解答以下各题：
将 $\scriptstyle Q \left( m , - m ^ { 2 } + 2 m + 3 \right)$ 代入 $y = k ^ { \prime } { \bigl ( } x + 1 { \bigr ) }$ 得，  
$- m ^ { 2 } + 2 m + 3 = k ^ { \prime } { \left( m + 1 \right) }$   
解得， $k ^ { \prime } = 3 - m$ ，  
∴ $A Q$ 的解析式为 $y = \left( 3 - m \right) \left( x + 1 \right)$ ，  
当 $x = 1$ 时， $y = 2 { \bigl ( } 3 - m { \bigr ) } = 6 - 2 m$ ，  
则 $M \left( 1 , 6 - 2 m \right)$ ，即 $M E = 6 - 2 m$ ，  
同理可得，直线 $B Q$ 的解析式为 $y = - ( m + 1 ) ( x - 3 )$ ，  
当 $x = 1$ 时， $y = 2 \left( m + 1 \right) = 2 m + 2$ ，  
则 $N \left( 1 , 2 m + 2 \right)$ ，即 $N E = 2 m + 2$ ，  
$\cdot M E + N E = 8$ ，  
$\cdot \ M E + N E$ 的值为定值，定值为 8
# 2023·四川乐山·统考二模
