【详解】（1）解：∵ $A ( - 2 , 0 )$ ， $B ( 4 , 0 )$ 在二次函数的图像上，  
∴将 $\cdot$ ， $\cdot$ 点代入二次函数表达式中，  
得 $\left\{ \begin{array} { c } { 4 a + \left( - 2 \right) b + 4 = 0 } \\ { 1 6 a + 4 b + 4 = 0 } \end{array} \right.$ , 解得 $\left\{ { \begin{array} { l } { \displaystyle a = - { \frac { 1 } { 2 } } } \\ { \displaystyle b = 1 } \end{array} } \right.$   
∴二次函数的表达式为 $y = - \frac { 1 } { 2 } x ^ { 2 } + x + 4$ ，将其化为顶点式为 $y = - \frac { 1 } { 2 } { \bigl ( } x - 1 { \bigr ) } ^ { 2 } + \frac { 9 } { 2 }$   
∴顶点 $\cdot$ 的坐标为 $\left( 1 , { \frac { 9 } { 2 } } \right)$   
（2）解：如图，过点 $\cdot$ 作 $P G \bot x$ 轴于点 $\cdot$ ，设点 $P$ 的坐标为 $\left( t , - { \frac { 1 } { 2 } } t ^ { 2 } + t + 4 \right)$   
