例31 请解答以下各题：
$\therefore P Q = - t ^ { 2 } + 2 t + 3 - ( - { \frac { 1 } { 3 } } t ^ { 2 } + { \frac { 2 } { 3 } } t + 1 ) = - { \frac { 2 } { 3 } } t ^ { 2 } + { \frac { 4 } { 3 } } t + 2 \ ,$   
$Q E = - { \frac { 1 } { 3 } } t ^ { 2 } + { \frac { 2 } { 3 } } t + 1 \qquad { \frac { P Q } { Q E } } = { \frac { - { \frac { 2 } { 3 } } t ^ { 2 } + { \frac { 4 } { 3 } } t + 2 } { - { \frac { 1 } { 3 } } t ^ { 2 } + { \frac { 2 } { 3 } } t + 1 } } = 2$   
PQ  
∴ $\mathcal { Q } E$ 的值为定值，该定值为 2
# 2023 福建厦门一中模拟
