【详解】（1）解：∵抛物线 $y = x ^ { 2 } + m x + n$ 经过 $\left( 0 , - 3 \right) , \left( 2 , - 3 \right)$ 两点，  
$\therefore \left\{ { \begin{array} { l } { - 3 = n } \\ { - 3 = 2 ^ { 2 } + 2 m + n } \end{array} } \right.$ 解得： $\begin{array} { c } { { \left\{ n = - 3 \right. } }  \\ { { \left. m = - 2 \right. } } \end{array}$   
∴抛物线的解析式为 $y { = } x ^ { 2 } - 2 x - 3$

（2） $\frac { S _ { \triangle A D E } } { S _ { \triangle B D C } }$ 是定值，定值为 $\frac { 1 } { 9 }$ ， 理由如下：

![](<../../qs_image_DB/专题3-1_二次函数中的10类定值、定点问题（解析版）/6e6d5b538917ac869f1183cf958ae67e84cea0e5d40fb36ed19d1f8b3070af93.jpg>)

设直线 $A C$ 的解析式为 $y = k x + b$ ,将 $A \left( - 1 , 0 \right)$ ， $C \left( t , t ^ { 2 } - 2 t - 3 \right)$ 代入 $y = k x + b$ ,可得 $\left\{ \begin{array} { l l } { 0 = - k + b } \\ { t ^ { 2 } - 2 t - 3 = k t + b } \end{array} \right.$ 解得 $\left\{ \begin{array} { l l } { k = t - 3 } \\ { b = t - 3 } \end{array} \right.$ ∴直线 $A C$ 的解析式为 $y = \left( t - 3 \right) x + \left( t - 3 \right)$ ，令 $x = 0$ ，则 $y = t - 3$ ，

$D ( 0 , \ t - 3 )$   
设直线 $B D$ 的解析式为 $y = m x + n$ ,  
将 $B \left( 3 , 0 \right)$ ， $D ( 0 , \ t - 3 )$ 代入 $y = m x + n$ ,  
可得 $\left\{ { \begin{array} { l } { 0 = 3 m + n } \\ { t - 3 = n } \end{array} } \right.$ 解得 $\left\{ { \begin{array} { l } { m = { \frac { 3 - t } { 3 } } } \\ { n = t - 3 } \end{array} } \right.$ ,  
∴直线 $B D$ 的解析式为 $y = \frac { 3 - t } { 3 } x + ( t - 3 )$ ，  
联立 $\left\{ y = { \frac { 3 - t } { 3 } } x + \left( t - 3 \right) \right.$ ， 解得 $x = 3$ 或 $x = - { \frac { t } { 3 } }$   
∴点 $E$ 的横坐标为 $- \frac { t } { 3 }$   
∴点 $\cdot$ 的纵坐标为： $\left( - \frac { t } { 3 } \right) ^ { 2 } - 2 \left( - \frac { t } { 3 } \right) - 3 = \frac { t ^ { 2 } } { 9 } + \frac { 2 t } { 3 } - 3$ ，$S _ { \scriptscriptstyle \mathrm { A } \scriptscriptstyle \mathrm { A } D E } = S _ { \scriptscriptstyle \mathrm { A } \scriptscriptstyle \mathrm { A } B E } - S _ { \scriptscriptstyle \mathrm { A } \scriptscriptstyle \mathrm { A } B D } = { \frac { 1 } { 2 } } A B \big ( y _ { D } - y _ { E } \big ) = { \frac { 1 } { 2 } } A B \Bigg [ t - 3 - \bigg ( { \frac { t ^ { 2 } } { 9 } } + { \frac { 2 t } { 3 } } - 3 \bigg ) \Bigg ] = A B \cdot { \frac { 3 t - t ^ { 2 } } { 1 8 } }$   
$\begin{array} { l } { { S _ { \scriptscriptstyle \mathrm { s B D C } } = S _ { \scriptscriptstyle \mathrm { s A B C } } - S _ { \scriptscriptstyle \mathrm { s A B D } } = \displaystyle \frac { 1 } { 2 } { \cal A } B \left( y _ { D } - y _ { C } \right) = \displaystyle \frac { 1 } { 2 } { \cal A } B \left[ t - 3 - \left( t ^ { 2 } - 2 t - 3 \right) \right] = { \cal A } B \cdot \displaystyle \frac { 3 t - t ^ { 2 } } { 2 } , } } \\ { { \displaystyle \mathrm { } } } \\ { { \therefore \displaystyle \frac { S _ { \scriptscriptstyle \mathrm { s A D E } } } { S _ { \scriptscriptstyle \mathrm { s B D C } } } = \displaystyle \frac { { \cal A } B \cdot \displaystyle \frac { 3 t - t ^ { 2 } } { 1 8 } } { { \cal A } B \cdot \displaystyle \frac { 3 t - t ^ { 2 } } { 2 } } = \displaystyle \frac { 1 } { 9 } . } } \end{array}$

# 2023 年福州市屏东中学中考模拟
