【答案】 $y = \frac { 1 } { 2 } x ^ { 2 } - x - \frac { 3 } { 2 }$ , (1,-2)$( 2 ) \frac { 3 } { 2 }$ 或 $- { \frac { 3 } { 2 } }$ (3)定值， $\angle E M F = 9 0 ^ { \circ }$ ，理由见详解【思路点拨】（1）将A 、 $B$ 代入解析式即可求解；

（2）可求直线 $y = k x - k$ 过定点 $G \big ( 1 , 0 \big )$ ，设 $F \left( m , \frac 1 2 m ^ { 2 } - m - \frac 3 2 \right) \_ E \left( n , \frac 1 2 n ^ { 2 } - n - \frac 3 2 \right) \ O \left( m ^ { 2 } \right)$ ，则有 $F \left( m , k m - k \right)$ ，

$E { \big ( } n , k n - k { \big ) }$ ， 可求 $\frac { E G } { F G } = \frac { 1 } { 4 }$ 或 $\frac { E G } { F G } = 4$ ， $\cdot$ 当 $\frac { E G } { F G } = \frac { 1 } { 4 }$ 时，过 $F$ 作 $F P \bot G M$ 交 $G M$ 于 $P$ ， 过 $E$ 作$E Q \bot G M$ 交 $G M$ 于 $\mathcal { Q }$ ，可求 $\left\{ \begin{array} { l } { { k m - k = - 4 \left( k n - k \right) } } \\ { { \displaystyle { \frac { 1 } { 2 } m ^ { 2 } - m - \frac { 3 } { 2 } = - 4 \left( \frac { 1 } { 2 } n ^ { 2 } - n - \frac { 3 } { 2 } \right) } } } \end{array} \right.$ 从而可求 $\begin{array} { c } { { \left\{ m = 5 \right. } }  \\ { { \left. n = 0 \right. } } \end{array}$ 求得 $E { \Bigg ( } 0 , - { \frac { 3 } { 2 } } { \Bigg ) }$ ， ,接可求解； $\cdot$ 当 $\frac { E G } { F G } = 4$ 时，由 $\cdot$ 同理可求 $\left\{ { \begin{array} { l } { m = 2 } \\ { n = - 3 } \end{array} } \right.$ 即可求解；

（3）分别过 $E$ 、 $F$ 作 $y$ 轴的平行线交过 $M$ 作 $x$ 轴的平行线于 $C$ 、 $D$ ，可求 ${ \frac { 1 } { 2 } } x ^ { 2 } - x - { \frac { 3 } { 2 } } = k x - k$ ，从而可得 $\scriptstyle { \left\{ \begin{array} { l l } { m + n = 2 + 2 k } \\ { m n = 2 k - 3 } \end{array} \right. }$ 从而可求 $\textstyle { \big ( } m - 1 { \big ) } { \big ( } 1 - n { \big ) } = 4$ ， 可 得 $1 - n = \frac { 4 } { m - 1 }$ , 由 tan $\angle D M F = { \frac { M D } { F D } }$ 和tan $\angle C M E = { \frac { E C } { C M } }$ 可证 tan $\angle D M F =$ tan $\angle C M E$ ，从而可得 $\angle D M F = \angle C M E$ ，即可求证
