【答案】B
$\angle G E A = \tan \angle F G H = \frac { 1 } { 3 }$ $\angle G F A = \frac { 3 } { 4 }$ GF 5 10AE【简证】易知tan 故 tan FH , 10 9 10 3
![](<../../qs_image_DB/专题1-3_“12345”模型·选填压轴必备大招（共3种类型）（解析版）__/4403e1f2ec1a10793794f4c9bd656806ff4615427ab80896a72279939be015cb.jpg>)
【常规法详解】解：∵四边形 ABCD是边长为 4的正方形，  
$A B \ = \ A D \ = \ C D \ = \ C B \ = \ 4$ ， $\angle \mathrm { D } = \angle \mathrm { A } = \angle A B C$ ，  
∴ $\angle D = \angle C B E = 9 0 ^ { \circ }$ ，  
由翻折得 $C G = C E$ ， $G F = E F$ ， $C F$ 垂直平分 $E G$ ，  
在 $R t \triangle C D G$ 和 $R t { \triangle } C B E$ 中，  
$\left\{ { { C G = C E } \atop { C D = C B } } \right.$   
$\therefore R t \triangle C D G \cong R t \triangle C B E ( H L ) ,$ ，  
∴ $D G = B E = 2$ ，  
$\therefore A G = A D - D G = 4 - 2 = 2 ,$   
$\therefore A E = A B + B E = 4 + 2 = 6 ,$   
$E G = \sqrt { A G ^ { 2 } + A E ^ { 2 } } = \sqrt { 2 ^ { 2 } + 6 ^ { 2 } } = 2 \sqrt { 1 0 }$   
∵ $A G ^ { 2 } + A F ^ { 2 } = F G ^ { 2 }$ ，且 $A F = 6 - E F$ ，  
$\therefore 2 ^ { 2 } + ( 6 - E F ) ^ { 2 } = E F ^ { 2 } ,$ 解得 $E F = \frac { 1 0 } { 3 }$ ,  
$\therefore \frac { 1 } { 2 } E G \cdot F H = \frac { 1 } { 2 } E F \cdot A G = S _ { \scriptscriptstyle \triangle E F G } ,$ $\frac { 1 } { 2 } \times 2 \sqrt { 1 0 } F H = \frac { 1 } { 2 } \times \frac { 1 0 } { 3 } \times 2$ 解得 $F H = \frac { \sqrt { 1 0 } } { 3 }$
