【详解】解：（1）将 $\cdot$ （-3，0）和 $\cdot$ （1，0）代入抛物线解析式 $y = a x ^ { 2 } + b x + 3$ 中，可得：$\left\{ \begin{array} { l l } { 0 = 9 a - 3 b + 3 } \\ { 0 = a + b + 3 } \end{array} \right.$ 解得： $\left\{ \begin{array} { l l } { a = - 1 } \\ { b = - 2 } \end{array} \right.$   
∴抛物线解析式为 $\cdot$ ；  
（2）假设存在，设 $\cdot$ 点坐标为(-1， $\cdot$ 、点 $M \ ( m , \ n )$   
$n = - m ^ { 2 } - 2 m + 3$   
$\therefore M E = { \frac { 9 } { 2 } } - n = { \frac { 9 } { 2 } } - \left( - \mathbf { m } ^ { 2 } - 2 m + 3 \right) = \mathbf { m } ^ { 2 } + 2 \mathbf { m } + { \frac { 3 } { 2 } }$   
$M F = M E - { \frac { 1 } { 4 } } = m ^ { 2 } + 2 m + { \frac { 5 } { 4 } }$   
而 $M F = \sqrt { \left( m + 1 \right) ^ { 2 } + \left( - m ^ { 2 } - 2 m + 3 - t \right) ^ { 2 } }$   
$( m + 1 ) ^ { 2 } + \left( - m ^ { 2 } - 2 m + 3 - t \right) ^ { 2 } = \left( m ^ { 2 } + 2 m + \frac { 5 } { 4 } \right) ^ { 2 }$   
$\therefore \left( - m ^ { 2 } - 2 m + 3 - t \right) ^ { 2 } = \left( m ^ { 2 } + 2 m + { \frac { 5 } { 4 } } \right) ^ { 2 } - ( m + 1 ) ^ { 2 }$   
${ \begin{array} { l } { = \left( m ^ { 2 } + 3 m + { \cfrac { 9 } { 4 } } \right) \left( n ^ { 2 } + m + { \cfrac { 1 } { 4 } } \right) = \left( m + { \cfrac { 3 } { 2 } } \right) ^ { 2 } \left( m + { \cfrac { 1 } { 2 } } \right) ^ { 2 } = \left( m ^ { 2 } + 2 m + { \cfrac { 3 } { 4 } } \right) ^ { 2 } } \\ { \vdots } \\ { \cdot m ^ { 2 } - 2 m + 3 - t = \left( m ^ { 2 } + 2 m + { \cfrac { 3 } { 4 } } \right) } \end{array} }$   
$\therefore t - 3 = \frac { 3 } { 4 }$ ， 即 $t = \frac { 1 5 } { 4 }$

$$
\therefore F { \left( - 1 , { \frac { 1 5 } { 4 } } \right) } .
$$

# 四川自贡·中考真题
