【详解】解：延长 $C B$ 至 $\cdot$ ，使 $B E = B D$ ，连接 $A E$ ，设 $B D = a$ ，

![](<../../qs_image_DB/专题1-6_二倍角的解题策略：倍半角模型与绝配角（解析版）_/224739b17279e7a01d67215c1d9c6cc9811be2b687f47c3277f3c678ae2394b4.jpg>)

∵B  90 ，  
∴ $\angle A B D = \angle A B E$ ，  
∴Rt△ABD≌Rt△ABEHL ，  
∴E  ADE ， $A E = A D$ ，  
∵ $\angle C = 2 \angle B A D$ ，  
$\therefore \angle C = \angle E A D$ ，$\angle D = \angle C + \angle D A C$ ，  
$\therefore \angle E = \angle A D E = \angle E A C ,$ ，  
$\therefore A C = C E = 3 a$ ，  
∵ $\angle E = \angle A D E = \angle E A C$ ， $\angle C = \angle E A D$ ，  
$\therefore \triangle E C A \sim \triangle E A D$ ，${ \frac { C A } { A D } } { = } { \frac { A D } { E D } }$ , 即 $\frac { 3 a } { A D } = \frac { A D } { 2 a }$   
∴ $A D = { \sqrt { 6 } } a$ ，又 $A C = 3 a$ ，$\frac { A D } { A C } = \frac { \sqrt { 6 } a } { 3 a } = \frac { \sqrt { 6 } } { 3 }$ 故答案为： $\frac { \sqrt { 6 } } { 3 }$
