【详解】（1）证明： $\angle A D C = \angle B + \angle B C D$ ， $\angle A E C = \angle B + \angle B A E$ ，又 $\angle A D C = \angle A E C$ ，  
 $\angle B C D = \angle B A E$ 且 $\angle B = \angle B$ ，  
$\therefore _ { \Delta A B E } \sim _ { \Delta C B D } ( \mathrm { A A } )$ ，  
$\therefore { \frac { B D } { B C } } = { \frac { B E } { A B } }$   
即： $B D \cdot A B = B E \cdot B C$ ；  
（2）解： $\cdot$ 过点 $D$ 做 $D F$ ∥ $A E$ ，设 $O E = 4 k$ ，则 $A O = 6 k$ ，  
又 $D$ 为 $A B$ 中点且 $D F / / A E$ ，  
$\therefore D F = { \frac { 1 } { 2 } } A E = 5 k .$ ．  
$\therefore { \frac { O E } { D F } } { = } { \frac { C E } { C F } } { = } { \frac { 4 } { 5 } }$   
$\therefore C F = 5$ ，  
$\therefore E F = B F = 1 , B C = 6 ,$   
又 $B D \cdot A B = B E \cdot B C$ ，  
$\therefore \frac { 1 } { 2 } A B \cdot A B = 2 \cdot 6$ ，  
解得： $A B = 2 { \sqrt { 6 } }$ ；  
$\cdot$ 过点A做 $A G \bot B C$ ，垂足为点 $G$ ，  
 $\triangle A E C$ 为等腰直角三角形，  
 $\angle A C E = \angle A E C = \angle A D C = 4 5 ^ { \circ }$ 且 $\angle D A C = \angle C A B$ ，  
$\therefore \triangle B A C \sim \triangle C A D$ ，${ \frac { A C } { B A } } { = } { \frac { A D } { A C } }$ ,  
又 $A B = 2 A D$ ，  
 $\cdot \ A B = { \sqrt { 2 } } A C = 4 \ ;$ ，  
在 $\mathrm { R t } \triangle A B G$ 中，  
$\begin{array} { r l } & { \mathrm { ~ \forall ~ } A B = 2 A G = 4 , } \\ & { \mathrm { ~ : ~ } \mathcal { L } M B G = 3 0 ^ { \circ } , } \\ & { \mathrm { ~ : ~ } B G = 2 \sqrt { 3 } , } \\ & { \mathrm { ~ : ~ } B G = 2 \sqrt { 3 } , } \\ & { \mathrm { ~ : ~ } S _ { S , \mathrm { a r g e } } = \frac { 1 } { 2 } S _ { S , \mathrm { a r d c } } = \frac { 1 } { 2 } \cdot \frac { 1 } { 2 } \cdot B G \cdot A G = \sqrt { 3 } + 1 , } \\ & { \mathrm { ~ : ~ } \mathcal { L } M B = 2 A G = 3 0 ^ { \circ } , } \\ & { \mathrm { ~ : ~ } S _ { S , \mathrm { a r g e } } = \frac { 1 } { 2 } \cdot A O \cdot A C = \frac { 4 \sqrt { 3 } } { 3 } , } \\ & { \mathrm { ~ : ~ } S _ { S , \mathrm { a r g e } } = S _ { S , \mathrm { a r g e } } - S _ { S , \mathrm { a r g e } } = 4 - \frac { 4 \sqrt { 3 } } { 3 } , } \\ & { \mathrm { ~ : ~ } S _ { \mathrm { a r g e } } = S _ { S , \mathrm { a r g e } } - S _ { S , \mathrm { a r g e } } = 4 \cdot \frac { 1 } { \lambda } , } \\ &  \mathrm { ~ : ~ } \mathcal { ~ } \alpha \end{array}$   
$\therefore S _ { \perp \perp \perp \mathcal { U } K B D O E } = S _ { \triangle B D C } - S _ { \triangle E O C } = ( \sqrt { 3 } + 1 ) - \left( 4 - \frac { 4 \sqrt { 3 } } { 3 } \right) = \frac { 7 \sqrt { 3 } } { 3 } - 3 .$

![](<../../qs_image_DB/专题1-2_一文吃透相似三角形12个模型·共14类题型（解析版）/4545c19cdb65e17a4010658563fceeebbc61efff643a4954e778404fb4bcf446.jpg>)

![](<../../qs_image_DB/专题1-2_一文吃透相似三角形12个模型·共14类题型（解析版）/76010ec275b1cef196eeff810873977a82c3aa6261ac8898beb5158d0c900926.jpg>)
