【解析】∵ $\cdot$ ， $\mathrm { A D } { = } 4$ ，∴DE $= 6$ ， $\therefore C D = C E = 3 { \sqrt { 2 } }$   
由题意，△ADF∽△CEA， $\cdot \frac { A D } { D F } { = } \frac { C E } { A E }$   
$\frac { 4 } { D F } \frac { 3 \sqrt { 2 } } { 2 } \frac { 4 \sqrt { 2 } } { 3 }$   
$\therefore \mathrm { C F } = \frac { 5 \sqrt { 2 } } { 3 } = \frac { 5 } { 9 } C D .$   
$\frac { 5 } { 9 } \times \frac { 2 } { 3 } \times \frac { 2 } { 3 } \times \frac { 1 } { 3 } \times \frac { 2 } { 2 } \times 3 \sqrt { 2 } \times 3 \sqrt { 2 } \frac { 1 0 } { 3 }$
