【详解】（1）在菱形 ABCD中， $\angle A B C = 1 2 0 ^ { \circ }$ ，  
$\angle A B D = \angle D B C = 6 0 ^ { \circ } \qquad A B = A D$ ，  
∴ $\triangle A B D$ 是等边三角形．  
（2）过 $B$ 点作 $B P \perp A D$ ，垂足为 $\cdot$ ，  
$\cdot \angle A B P = 3 0 ^ { \circ }$ ，  
$A P = { \frac { 1 } { 2 } } A B = { \frac { 3 } { 2 } }$   
${ \begin{array} { l } { \displaystyle \therefore B P = { \sqrt { A B ^ { 2 } - A P ^ { 2 } } } = { \frac { 3 { \sqrt { 3 } } } { 2 } } , } \\ { \displaystyle \because A E = 1 , } \\ { \displaystyle \therefore P E = { \frac { 1 } { 2 } } , } \end{array} }$   
$\therefore B E = { \sqrt { B P ^ { 2 } + P E ^ { 2 } } } = { \sqrt { \left( { \frac { 3 { \sqrt { 3 } } } { 2 } } \right) ^ { 2 } + \left( { \frac { 1 } { 2 } } \right) ^ { 2 } } } = { \sqrt { 7 } } \ ,$   
∵将射线 $E B$ 绕点 $E$ 逆时针旋转 $\cdot$ ，得到线段 $E F$ ，  
∴ $. \angle B E F = 6 0 ^ { \circ }$ ，$. \angle A E B + \angle D E F = 1 2 0 ^ { \circ }$ ，  
又∵ $\angle A E B + \angle A B E = 1 2 0 ^ { \circ }$ ，  
$\cdot \angle A B E = \angle D E F$   
∵ $\triangle A B D$ 是等边三角形，  
∴ $\cdot \angle A = \angle A D B = 6 0 ^ { \circ } ,$ ，  
$\therefore \Delta D E G \sim \Delta A B E$ ，  
$\therefore { \frac { D G } { A E } } = { \frac { D E } { A B } } = { \frac { E G } { B E } } ,$   
$\therefore { \frac { D G } { 1 } } = { \frac { 2 } { 3 } } = { \frac { E G } { \sqrt { 7 } } } ,$   
$\therefore D G = { \frac { 2 } { 3 } } , E G = { \frac { 2 { \sqrt { 7 } } } { 3 } } .$   
（3）设 $A B = m$ ， $A E = n$ ，  
如图，过 $\cdot$ 点作 $E H / / A B$ 交 $D B$ 于 $H$ ，  
∴ $\angle A = D E H = 6 0 ^ { \circ }$ ，  
∴ $\triangle D E H$ 是等边三角形，$. D H = E H = D E = m - n$ ，  
由（2）知 $\triangle D E G \sim \triangle A B E$ ，  
$\frac { D G } { A E } = \frac { D E } { A B }$   
${ \frac { D G } { n } } = { \frac { m - n } { m } }$   
∴ DG n  m n  mDG 4BG 21DG 4B D 254  
∴DG 25 m，  
${ \frac { n { \bigl ( } m - n { \bigr ) } } { m } } = { \frac { 4 } { 2 5 } } m$ ，∴ $n = \frac { 4 m } { 5 }$ 或 $n = \frac { m } { 5 }$   
∵ EH∥AB ，  
∴ EH∥DF ，  
$\therefore \frac { E G } { G F } = \frac { H G } { D G } = \frac { D H - D G } { D G } = \frac { m - n - \displaystyle \frac { 4 m } { 2 5 } } { \displaystyle \frac { 4 m } { 2 5 } } = \frac { 2 1 m - 2 5 n } { 4 m } ,$   
当 $n = \frac { 4 m } { 5 }$ 时， $\frac { E G } { G F } = \frac { 2 1 m - 2 5 n } { 4 m } = \frac { 1 } { 4 }$   
当 $n = \frac { m } { 5 }$ 时， $\frac { E G } { G F } = \frac { 2 1 m - 2 5 n } { 4 m } = 4$ $\frac { E G } { G F }$ 的值为 $\frac { 1 } { 4 }$ 或4 ．

![](<../../qs_image_DB/专题1-2_一文吃透相似三角形12个模型·共14类题型（解析版）/52bbdb51f4e8d67d0926ae0fa5c8b4ab2bc03e807c80ace0edb038484c49fe2f.jpg>)

![](<../../qs_image_DB/专题1-2_一文吃透相似三角形12个模型·共14类题型（解析版）/59de55d276d100b030b199e5ec45779c212b7fb1cbc0c6c0d4508bd75f0e1454.jpg>)
