【详解】解：过点 $F$ 作 $M N / / C D$ ，交 $A D , B C$ 分别于 $M , N$ ，

![](<../../qs_image_DB/专题1-2_一文吃透相似三角形12个模型·共14类题型（解析版）/d969f9bd1d930c5414dae4c86c833eac7b1dff925717f16edeb6a6cd1188756b.jpg>)

∵四边形 $A B C D$ 为矩形，  
∴四边形DCNM 和四边形AMNB均为矩形，  
∴ $. \angle D M F = \angle F N G = \angle F M A = \angle E A B = 9 0 ^ { \circ } , ~ C D = M N = A B , ~ D M = C N ;$ ；  
$\mathbf { R t } \triangle B E F$ 和 $\mathrm { R t } \triangle D F G$ 是一副三角尺，  
$D F = F G , \angle D F G = \angle F E B = 9 0 ^ { \circ } , \angle F B E = 3 0 ^ { \circ }$   
$: \angle M F D + \angle M D F = \angle G F N + \angle M F D = 9 0 ^ { \circ } , \angle B E A + \angle M F E = \angle A B E + \angle B E A = 9 0 ^ { \circ } ,$   
∴ $\angle M D F = \angle G F N , \angle M F E = \angle A B E$ ，  
${ \scriptstyle \triangle D M F { \cong } \triangle F N G ( A A S ) }$ ，  
$\therefore D M = F N , M F = G N$ ，  
设 $D M = x , M F = y$ ，  
则： $D M = F N = x , M F = G N = y$ ，  
∴ ${ \cal D } F ^ { 2 } = { \cal D } M ^ { 2 } + M F ^ { 2 } = x ^ { 2 } + y ^ { 2 } , { \cal D } G ^ { 2 } = { \cal D } F ^ { 2 } + F G ^ { 2 } = 2 { \cal D } F ^ { 2 } = 2 x ^ { 2 } + 2 y ^ { 2 } , { \cal M } N = F M + F N = x + y ,$ ，∵ $B E = D G$ ，  
$B E ^ { 2 } = 2 x ^ { 2 } + 2 y ^ { 2 }$ ，  
∵ $\angle F M A = \angle E A B , \angle M F E = \angle A B E$ ，  
∴FME∽EAB ，$\cdot \frac { M F } { A E } { = } \frac { E F } { B E }$ ,  
∵FBE  30，  
${ \begin{array} { l } { E F = { \cfrac { 1 } { 2 } } B F , B E = { \sqrt { B F ^ { 2 } - E F ^ { 2 } } } = { \frac { \sqrt { 3 } } { 2 } } B F } \\ { { \cfrac { M F } { A E } } = { \frac { E F } { B E } } = { \cfrac { 1 } { \sqrt { 3 } } } } \\ { A E = { \sqrt { 3 } } M F = { \sqrt { 3 } } y } \\ { A B ^ { 2 } = B E ^ { 2 } - A E ^ { 2 } = 2 x ^ { 2 } + 2 y ^ { 2 } - 3 y ^ { 2 } = 2 x ^ { 2 } - y ^ { 2 } } \\ { M N = A B } \end{array} }$   
$\left( x + y \right) ^ { 2 } = 2 x ^ { 2 } - y ^ { 2 }$ ，即： $x ^ { 2 } - 2 x y - 2 y ^ { 2 } = 0$ ，  
∴ $x = \left( 1 + { \sqrt { 3 } } \right) y$ 或 $x = \left( 1 - { \sqrt { 3 } } \right) y$ （不符合题意，舍去），  
$C D = M N = x + y = \left( 2 + { \sqrt { 3 } } \right) y , C G = C N - G N = D M - G N = x - y = { \sqrt { 3 } } y$ ，  
$\frac { D C } { C G } = \frac { \left( 2 + \sqrt { 3 } \right) y } { \sqrt { 3 } y } = \frac { \left( 2 + \sqrt { 3 } \right) } { \sqrt { 3 } } = \frac { 2 \sqrt { 3 } } { 3 } + 1$
