【详解】（1）解： $\triangle B D E \sim \triangle C F D$ ，理由如下：  
∵如图 1， $\angle B = \angle C = \angle E D F$ ，  
$\angle E D C = \angle B + \angle B E D = \angle E D F + \angle F D C$ ，  
∴ $\angle B E D = \angle F D C$ ，  
$\triangle B D E \sim \triangle C F D$ ，

![](<../../qs_image_DB/专题1-2_一文吃透相似三角形12个模型·共14类题型（解析版）/40c9bd09cb63344d3094dca272d9f9ffc184be141e7e6f72abe6043b79e0535b.jpg>)  
图1

（2） $\cdot$ 如图 2，设 $\boldsymbol { A } \boldsymbol { E } = \boldsymbol { x } , \boldsymbol { A } \boldsymbol { F } = \boldsymbol { y }$ ，

![](<../../qs_image_DB/专题1-2_一文吃透相似三角形12个模型·共14类题型（解析版）/d6fe83b47eb77e05759a38cfc899f251edfb0c9038acfb0be284ecefac316f3f.jpg>)  
图2

∵ ${ \triangle A B C }$ 为等边三角形，其边长为 8， $B D = 2$ ，$\cdot \angle A = \angle B = \angle C , A B = A C = B C = 8$ ，  
则 $B E = 8 - x , C F = 8 - y , C D = 6$   
∵ $\triangle E D F$ 是由 $\triangle A E F$ 沿 $E F$ 翻折得到，  
∴ $\angle B = \angle C = \angle E D F = \angle A , D E = A E = x$ $\cdot \angle E D C = \angle B + \angle B E D = \angle E D F + \angle F D C$   
∴ $. \angle B E D = \angle F D C$ ，  
$\therefore \triangle B D E \sim \triangle C F D ,$ ，  
$\therefore \frac { D E } { F D } = \frac { B E } { C D } = \frac { B D } { C F } , \textcircled { \ast } \frac { x } { y } = \frac { 8 - x } { 6 } = \frac { 2 } { 8 - y } ,$   
解得 ${ \frac { x } { y } } = { \frac { 5 } { 7 } }$ , 即 ${ \frac { A E } { A F } } = { \frac { 5 } { 7 } }$   
$\textcircled{2}$ 如图 3，设 $\boldsymbol { A } \boldsymbol { E } = \boldsymbol { x } , \boldsymbol { A } \boldsymbol { F } = \boldsymbol { y }$ ，  
∵ ${ \triangle A B C }$ 为等边三角形，其边长为 8， $B D = 2$ ，  
∴ $\angle A = \angle A B C = \angle A C B = 6 0 ^ { \circ } , A B = A C = B C = 8$ ，  
∴ $\angle D B E = \angle F C D = 1 2 0 ^ { \circ } , D C = 1 0$ ，  
又∵ $\triangle E D F$ 是由 $\triangle A E F$ 沿 $E F$ 翻折得到，  
∴ $\angle E D F = \angle A = \angle E B C = 6 0 ^ { \circ } , D E = A E = x , D F = A F = y , B E = 8 - x , C F = y - 8$ ，  
又∵ $\angle E B C = \angle B E D + \angle B D E , \angle E D F = \angle C D F + \angle B D E ,$   
∴ $\angle B E D = \angle C D F$ ，  
$\triangle B D E \sim \triangle C F D$ $ { \frac { D E } { D F } } = { \frac { B E } { C D } } = { \frac { B D } { C F } }$ 即 ${ \frac { x } { y } } = { \frac { 8 - x } { 1 0 } } = { \frac { 2 } { y - 8 } }$ ${ \frac { x } { y } } = { \frac { 1 } { 3 } }$ $\frac { D E } { F D } { = } \frac { A E } { A F } { = } \frac { 1 } { 3 }$ BDES △ DE 1即CFDS △ FD 9

![](<../../qs_image_DB/专题1-2_一文吃透相似三角形12个模型·共14类题型（解析版）/4a9c5fd786ba4414b628bf3a481bce4784bf2e091eeb55972bced4af12b140a6.jpg>)  
图3

# 2023·湖北武汉·统考中考真题
