【答案】 $\frac { 3 { \sqrt { 2 } } - { \sqrt { 6 } } } { 6 }$ 【详解】解：连接 $A D$ ，

![](<../../qs_image_DB/专题1-2_一文吃透相似三角形12个模型·共14类题型（解析版）/afbe814156076300aadc0d9804b95ee862d1d17a7894886843b293f540f60731.jpg>)

∵将 $A C$ 绕着点 $C$ 按顺时针旋转 $6 0 ^ { \circ }$ 得到 $C D$   
∴ $A C = C D$ ，  
$\therefore \triangle A C D$ 是等边三角形，  
∴ $A C = A D = C D$ ， $\angle A D C = \angle C A D = 6 0 ^ { \circ } ,$   
设 $A C = A D = C D = a$ ，则 $A B = A C = a$ ，  
取 $A C$ 的中点 $\cdot$ ，连接 $D H$ ，  
$A H = C H = \frac { 1 } { 2 } A C = \frac { 1 } { 2 } a \angle A H D = 9 0 ^ { \circ }$   
$D H = { \frac { \sqrt { 3 } } { 2 } } a$   
设 $A E = x$ ，则 $E H = A H - A E = { \frac { 1 } { 2 } } a - x$ ，$\angle B A C = 9 0 ^ { \circ }$ ，  
∴ $. \angle B A E = \angle D H E$ ，  
∵ $\angle A E B = \angle H E D$ ，  
$\therefore \Delta A E B \sim _ { \Delta } H E D$ ，$\cdot \frac { A E } { H E } { = } \frac { A B } { D H } .$ ,  
${ \frac { x } { { \frac { 1 } { 2 } } a - x } } = { \frac { a } { \frac { \sqrt { 3 } } { 2 } a } } \quad$   
解得 $x = \left( 2 - { \sqrt { 3 } } \right) a$ ，  
即 $A E = { \bigg ( } 2 - { \sqrt { 3 } } { \bigg ) } a$ ，  
$\begin{array} { l l l } { { \dot { \cdot } \ E H = A H - A E = { \displaystyle { \frac { 1 } { 2 } } } a - x = { \displaystyle { \frac { 1 } { 2 } } } a - \left( 2 - \sqrt { 3 } \right) a = { \displaystyle { \frac { 2 \sqrt { 3 } - 3 } { 2 } } } a \ , } } & { { } } \\ { { \dot { \cdot } \ D L E ^ { 2 } = 3 \left( 2 - \sqrt { 3 } \right) a ^ { 2 } \ , } } & { { } } & { { } } \\ { { \dot { \cdot } \quad \frac { A E } { E D } = \sqrt { \displaystyle { \frac { A E ^ { 2 } } { E D ^ { 2 } } } } \quad } } & { { = \sqrt { \displaystyle { \frac { \left( 2 - \sqrt { 3 } \right) ^ { 2 } a ^ { 2 } } { 3 \left( 2 - \sqrt { 3 } \right) a ^ { 2 } } } } \quad } } & { { = \sqrt { \displaystyle { \frac { 2 - \sqrt { 3 } } { 3 } } } \quad } } & { { = \frac { \sqrt { 6 - 3 \sqrt { 3 } } } { 3 } } } & { { = \frac { \sqrt { \displaystyle { \frac { 2 4 - 1 2 \sqrt { 3 } } { 4 } } } } { 3 } } } \\ { { \dot { \phantom { \frac { 2 } { 5 } } } \quad } } & { { { \displaystyle { \frac { \sqrt { 3 } } { E D } } } } } & { { = \sqrt { \displaystyle { \frac { \left( 2 - \sqrt { 3 } \right) a ^ { 2 } } { 3 \left( 2 - \sqrt { 3 } \right) a ^ { 2 } } } } \quad } } & { { = \sqrt { \displaystyle { \frac { 2 - \sqrt { 3 } } { 3 } } } \quad } } & { { = \frac { \sqrt { 6 - 3 \sqrt { 3 } } } { 3 } } } & { { = \frac { \sqrt { \displaystyle { \frac { 2 4 - 1 2 \sqrt { 3 } } { 4 } } } } { 3 } } } \end{array} \quad \nonumber  \displaystyle { \begin{array} { l } { { \dot { \sqrt { 2 } } \dot { \ \sigma } _ { \mu } ^ { 2 } } } \\ { { \dot { \sqrt { 3 } } \dot { \sigma } _ { \mu } ^ { 2 } } } \end{array} }$ 18 12 3 6 43  
$= { \frac { \sqrt { \frac { \left( 3 { \sqrt { 2 } } \right) ^ { 2 } - 2 \times 3 { \sqrt { 2 } } \times { \sqrt { 6 } } + \left( { \sqrt { 6 } } \right) ^ { 2 } } { 4 } } } { 3 } } = { \frac { \sqrt { \frac { \left( 3 { \sqrt { 2 } } - { \sqrt { 6 } } \right) ^ { 2 } } { 4 } } } { 3 } } = { \frac { 3 { \sqrt { 2 } } - { \sqrt { 6 } } } { 6 } }$
