【详解】问题背景： $\triangle A B C \sim \triangle A D E$ ，∴∠BAC=∠DAE， $\frac { A B } { A D } { = } \frac { A C } { A E }$ ,  
$-$ ，  
∴∠BAD $\cdot$ ∠CAE，  
$\therefore \Delta A B D \sim \Delta A C E$ ；  
尝试应用：连接 CE，  
∵ $\angle B A C = \angle D A E = 9 0 ^ { \circ }$ ， $\angle A B C = \angle A D E = 3 0 ^ { \circ }$ ，  
$\therefore \Delta B A C \sim \Delta D A E$ ，$\cdot \frac { A B } { A C } { = } \frac { A D } { A E }$ ，  
$\therefore \angle B A D + \angle D A C = \angle A E + \angle D A C ,$ ，  
$-$ ，  
$\therefore \Delta A B D \sim \Delta A C E$ ，$\ { \frac { B D } { C E } } { = } { \frac { A D } { A E } }$   
由于 $\angle A D E = 3 0 ^ { \circ } , \angle D A E = 9 0 ^ { \circ }$ ，  
$\therefore t a n 3 0 ^ { \circ } = { \frac { A E } { A D } } = { \frac { \sqrt { 3 } } { 3 } } ,$   
即 ${ \frac { B D } { C E } } { = } { \frac { A D } { A E } } { = } { \sqrt { 3 } }$ ，  
$\because \frac { A D } { B D } = \sqrt { 3 }$ ，$\cdot \frac { A D } { C E } { = 3 }$ ，  
$\because \angle B A C = \angle D A E = 9 0 ^ { \circ } , \angle A B C = \angle A D E = 3 0 ^ { \circ } ,$ ，  
∴ $\angle C = \angle E = 6 0 ^ { ^ { \circ } }$ ，  
又∵ $\angle A F E = \angle D F C$ ，  
$\triangle A F E \sim \triangle D F C$ ，${ \frac { A F } { D F } } { = } { \frac { E F } { C F } }$ 即 $\frac { A F } { E F } { = } \frac { D F } { C F }$   
又∵ $\angle A F D = \angle E F C$   
$\therefore \triangle A D F ^ { \sim } \triangle E C F$ ，$\frac { D F } { C F } { = } \frac { A D } { C E } { = } 3$   
拓展创新： $A D = { \sqrt { 5 } }$   
如图，在 AD 的右侧作 $-$ ，AE 交 B

![](<../../qs_image_DB/专题1-2_一文吃透相似三角形12个模型·共14类题型（解析版）/e30db191119e601969649ea1da44cb46ce15036f56f1fb3d0e20d1535e87e76c.jpg>)

![](<../../qs_image_DB/专题1-2_一文吃透相似三角形12个模型·共14类题型（解析版）/4a1b6cf186de782dea39ddb141cb5f4c5b534db8b00a94756118bfb80b0432f2.jpg>)

∵∠ADE ∠BAD+∠ABD，∠ABC $\varprojlim 2$ ∠ABD+∠CBD， $\angle B A D = \angle C B D = 3 0 ^ { \circ }$ ，

∴∠ADE=∠ABC，  
又∵∠DAE=∠BAC，  
$\therefore \Delta B A C \sim \Delta D A E$ ，  
${ \frac { A B } { A D } } { = } { \frac { A C } { A E } } { = } { \frac { B C } { D E } }$   
又∵ $-$ ，  
$-$ ，  
∴BAD∽CAE ，  
$\therefore { \frac { B D } { C E } } = { \frac { A B } { A C } } = { \frac { A D } { A E } } = { \frac { 4 } { 2 { \sqrt { 3 } } } } = { \frac { 2 { \sqrt { 3 } } } { 3 } } ,$   
设 $\mathrm { C D } { = } \mathbf { x }$ ，在直角三角形 BCD 中，由于 $\angle C \mathrm { B D } { = } 3 0 ^ { \circ }$ ，  
$\therefore B D = \sqrt { 3 } x , B C = 2 x , \therefore C E = \frac { 3 } { 2 } x , \therefore D E = \sqrt { ( \frac { 3 } { 2 } x ) ^ { 2 } - x ^ { 2 } } = \frac { \sqrt { 5 } } { 2 } x ,$ ，  
$\because { \frac { A B } { A D } } = { \frac { B C } { D E } } , { \therefore } { \frac { 4 } { A D } } = { \frac { 2 x } { \frac { \sqrt { 5 } } { 2 } x } } , { \therefore A D } = { \sqrt { 5 } }$
