【详解】解：（1）∵ DE⊥ AB， $D F \bot A C$ ， $\angle A = 9 0 ^ { \circ }$ ，$. D E / / A C$ ， $D F / / A B$ ，  
点 $D$ 是 $B C$ 的中点，  
 $D E$ ， $D F$ 是 ${ \triangle A B C }$ 的中位线，  
$\therefore D E = \frac { 1 } { 2 } A C = 2 , D F = \frac { 1 } { 2 } A B = 1 ,$   
则 $\frac { D E } { D F } = 2$ ，故答案为：2；

（2）如图 2，过点 $D$ 作 $D M \perp A B$ 于点 $M$ ，作 $D N \perp A C$ 于点 $N$ ，

![](<../../qs_image_DB/专题1-2_一文吃透相似三角形12个模型·共14类题型（解析版）/3f6414ba1b2ce4bc84c5c07ebb6b1e3104d8068abad3ec2ad2a9fa203fc5dab0.jpg>)  
图2

则 $\angle D M E = \angle D N F = \angle A = 9 0 ^ { \circ }$ ，  
 $\angle M D N = 9 0 ^ { \circ }$ ，即 $\angle M D E + \angle E D N = 9 0 ^ { \circ }$ ，$\cdot D E \bot D F$ ，  
 $\angle E D F = 9 0 ^ { \circ }$ ，即 $\angle E D N + \angle N D F = 9 0 ^ { \circ }$ ，  
 $. \angle M D E = \angle N D F$ ，  
$\cdot _ { \triangle } D M E ^ { \sim } { } _ { \triangle } D N F$ ，$\cdot \frac { D E } { D F } { = } \frac { D M } { D N }$ ,

由（1）知， $\frac { D M } { D N } = 2$ $\frac { D E } { D F } = 2$ ， 故答案为：2；

（3）如图 3，过点 $P$ 作 $D P \bot A B$ 于点 $P$ ， $D Q \bot A C$ 于点 $\boldsymbol { Q }$ ，

![](<../../qs_image_DB/专题1-2_一文吃透相似三角形12个模型·共14类题型（解析版）/e18c84c1c0800998a21b3e10a3cd0cbe4106ebc111716edd5c574100e4176d7d.jpg>)  
图3

$. \angle D P A = \angle D Q A = \angle A = 9 0 ^ { \circ }$ ， DP∥AC ， DQ∥AB ，四边形 $A P D Q$ 是矩形，  
 $D P = A Q$ ， $D Q = A P$ ，  
$\therefore { \frac { C D } { B D } } = { \frac { a } { b } }$ ,  
$\therefore { \frac { C D } { C B } } = { \frac { a } { a + b } } B D = { \frac { b } { a + b } }$   
Q DP∥AC ，  
$\therefore \Delta D Q C \sim _ { \Delta } B A C$ ，  
$\therefore { \frac { D Q } { A B } } = { \frac { C D } { C B } } ,$   
DQ∥AB，  
$\therefore \Delta D P B \sim \Delta C A B$ ，  
$\therefore { \frac { D P } { A C } } = { \frac { B D } { B C } }$   
$\therefore D Q = { \frac { C D } { C B } } \cdot A B = { \frac { 2 a } { a + b } } , D P = { \frac { B D } { B C } } \cdot A C = { \frac { 4 b } { a + b } } ,$   
同（2）的方法知，知， $\frac { D E } { D F } = \frac { D P } { D Q } = \frac { \frac { 4 b } { a + b } } { \frac { 2 a } { a + b } } = \frac { 2 b } { a } ;$ ；  
（4）如图 3，连接 $E F$ ，  
