【详解】（1）证明：因为 $A D \cdot O C = A B \cdot O D$ ，  
所以 ${ \frac { A D } { A B } } { = } { \frac { O D } { O C } }$   
所以 ${ \frac { A D ^ { 2 } } { A B ^ { 2 } } } { = } { \frac { O D ^ { 2 } } { O C ^ { 2 } } }$ ,  
所以 ${ \frac { A D ^ { 2 } } { A B ^ { 2 } - A D ^ { 2 } } } = { \frac { O D ^ { 2 } } { O C ^ { 2 } - O D ^ { 2 } } }$   
因为 $B D$ 是 ${ \triangle A B C }$ 边 $A C$ 上的高，  
所以 $\angle A D B = \angle O D C = 9 0 ^ { \circ }$ ，  
所以 ${ \frac { A D ^ { 2 } } { B D ^ { 2 } } } { = } { \frac { O D ^ { 2 } } { C D ^ { 2 } } }$ 即 ${ \frac { A D } { B D } } { = } { \frac { O D } { C D } }$ ,  
所以 $\triangle A B D ^ { \circ } \triangle O C D$ ，  
所以 $\angle A B D = \angle A C E$ ，  
因为 $\angle A = \angle A$ ，  
所以 $\triangle A B D \sim \triangle A C E$

（2）证明：根据（1）得 $\triangle A B D \sim \triangle A C E$ ，所以 ${ \frac { A D } { A E } } { = } { \frac { A B } { A C } }$ ,所以 ${ \frac { A D } { A B } } { = } { \frac { A E } { A C } }$ ；

![](<../../qs_image_DB/专题1-2_一文吃透相似三角形12个模型·共14类题型（解析版）/a26ffebd446ab3bbad80c36804102defa7ed1965352c7e86f3ab493ccaf9691a.jpg>)

因为 $\angle D A E = \angle B A C$ ，所以 $\triangle D A E \sim \triangle B A C$ ，因为 $A F$ 平分 $\angle B A C$ ，所以 ${ \frac { D E } { B C } } { = } { \frac { A G } { A F } }$ 所以 $A F \cdot D E = A G \cdot B C$
