【详解】（1）解：由题知， $A B = B C = C D = D A = 1$ ，  
若 $E D = \frac { 1 } { 3 }$ 则 $A E = A D - E D = \frac { 2 } { 3 }$   
四边形 ABCD是正方形，  
 $\angle A = \angle F D E = 9 0 ^ { \circ }$ ，  
又 $\angle A E B = \angle F E D$ ，  
$\therefore \triangle A E B \sim \triangle D E F$ ，  
$\therefore { \frac { A B } { D F } } = { \frac { A E } { E D } }$   
即 $\mathrm { ~  ~ \imath ~ } \frac { 1 } { D F } { = } \frac { \displaystyle \frac { 2 } { 3 } } { \displaystyle \frac { 1 } { 3 } } ,$   
$\therefore D F = { \frac { 1 } { 2 } }$ （2）证明：四边形 $A B C D$ 是正方形，  
 $\angle A = \angle C = 9 0 ^ { \circ }$ ， $A B / / C D$ ，$\cdot \angle A B E = \angle F$ ，  
$\therefore \triangle A B E \sim _ { \triangle } C F B$ ，$\cdot \frac { A B } { C F } { = } \frac { A E } { B C }$   
 $\cdot \ A E \cdot C F = A B \cdot B C = 1 \times 1 = 1$   
（3）解：设 $E G = E D = x$ ，  
