【详解】解： $y = - x ^ { 2 } - 2 x + 3 = - { \bigl ( } x + 1 { \bigr ) } ^ { 2 } + 4$ ，  
∴当 $x < - 1$ 时， $\cdot$ 随 $\cdot$ 的增大而增大，当 $x > - 1$ 时， $\cdot$ 随 $\cdot$ 的增大而减小，若 $a \geq - 1$ ，当 $a \bullet x \bullet { \frac { 1 } { 2 } }$ 时， $y$ 随 $\cdot$ 的增大而减小，  
此时当 $x = \frac { 1 } { 2 }$ 时，函数值 $\cdot$ 最小，最小值为 $\frac { 7 } { 4 }$ , 不合题意，  
若 $a < - 1$ ，当 $x = a$ 时，函数值 $y$ 最小，最小值为 1，  
$- a ^ { 2 } - 2 a + 3 = 1$ ，  
解得： $a = - 1 - { \sqrt { 3 } }$ 或 $- 1 + { \sqrt { 3 } }$ （舍去）；  
综上所述， $\cdot$ 的值为 $- 1 - { \sqrt { 3 } }$   
故答案为： $- 1 - { \sqrt { 3 } }$

# 2023·湖北十堰中考真题
